<?xml version="1.0" encoding="UTF-8"?>
<rdf:RDF
   xmlns="https://www.scss.tcd.ie/~kamarajk/EthicsOntology#"
   xmlns:owl="http://www.w3.org/2002/07/owl#"
   xmlns:rdf="http://www.w3.org/1999/02/22-rdf-syntax-ns#"
   xmlns:rdfs="http://www.w3.org/2000/01/rdf-schema#"
>
  <rdf:Description rdf:about="https://www.scss.tcd.ie/~kamarajk/EthicsOntology#hasHealthData">
    <rdfs:comment xml:lang="en">Information about the data subject's health, medical conditions or health care (medical history, test results, etc.) is present. This data property was inspired by the "dpv:MedicalHealth" class in the Data Privacy Vocabulary (DPV).</rdfs:comment>
    <rdf:type rdf:resource="http://www.w3.org/2002/07/owl#DatatypeProperty"/>
    <rdfs:range rdf:resource="http://www.w3.org/2001/XMLSchema#boolean"/>
    <rdfs:domain rdf:resource="https://www.scss.tcd.ie/~kamarajk/EthicsOntology#Group"/>
    <rdfs:seeAlso>https://www.w3.org/ns/dpv#dpv:MedicalHealth</rdfs:seeAlso>
    <rdfs:domain rdf:resource="https://www.scss.tcd.ie/~kamarajk/EthicsOntology#Individual"/>
  </rdf:Description>
  <rdf:Description rdf:about="https://www.scss.tcd.ie/~kamarajk/EthicsOntology#isChild">
    <rdf:type rdf:resource="http://www.w3.org/2002/07/owl#DatatypeProperty"/>
    <rdfs:range rdf:resource="http://www.w3.org/2001/XMLSchema#boolean"/>
    <rdfs:domain rdf:resource="https://www.scss.tcd.ie/~kamarajk/EthicsOntology#Group"/>
    <rdfs:comment xml:lang="en">The data subject is a child. This data property was inspired by the "dpv:Child" class in the Data Privacy Vocabulary (DPV).

According to DPV:

- A 'child' is a natural legal person who is below a certain legal age depending on the legal jurisdiction.

- A 'child' is distinct from a 'minor'. For example, the legal age for a 'minor' in most countries is 18, whereas a 'child' can be a minor below the age of 14.</rdfs:comment>
    <rdfs:seeAlso>https://www.w3.org/ns/dpv#dpv:Child</rdfs:seeAlso>
    <rdfs:domain rdf:resource="https://www.scss.tcd.ie/~kamarajk/EthicsOntology#Individual"/>
  </rdf:Description>
  <rdf:Description rdf:about="https://www.scss.tcd.ie/~kamarajk/EthicsOntology#hasEthnicityData">
    <rdfs:domain rdf:resource="https://www.scss.tcd.ie/~kamarajk/EthicsOntology#Individual"/>
    <rdfs:comment xml:lang="en">Information about the data subjectâ€™s origins and lineage is present. This data property was inspired by the "dpv:Ethnicity" class in the Data Privacy Vocabulary (DPV).

Ethicity data is any data that involves the data subject's ethnic origin, native language, race, caste, accent, dialect, or the immigration status of the data subject or their parents.</rdfs:comment>
    <rdfs:domain rdf:resource="https://www.scss.tcd.ie/~kamarajk/EthicsOntology#Group"/>
    <rdfs:range rdf:resource="http://www.w3.org/2001/XMLSchema#boolean"/>
    <rdf:type rdf:resource="http://www.w3.org/2002/07/owl#DatatypeProperty"/>
    <rdfs:seeAlso>https://www.w3.org/ns/dpv#dpv:Ethnicity</rdfs:seeAlso>
  </rdf:Description>
  <rdf:Description rdf:about="https://www.scss.tcd.ie/~kamarajk/EthicsOntology#hasIncomeData">
    <rdf:type rdf:resource="http://www.w3.org/2002/07/owl#DatatypeProperty"/>
    <rdfs:range rdf:resource="http://www.w3.org/2001/XMLSchema#boolean"/>
    <rdfs:seeAlso>https://www.w3.org/ns/dpv#income</rdfs:seeAlso>
    <rdfs:domain rdf:resource="https://www.scss.tcd.ie/~kamarajk/EthicsOntology#Individual"/>
    <rdfs:comment xml:lang="en">Information about the data subject's income is present. This data property was inspired by the "dpv:Income" class in the Data Privacy Vocabulary (DPV).</rdfs:comment>
  </rdf:Description>
  <rdf:Description rdf:about="https://www.scss.tcd.ie/~kamarajk/EthicsOntology#isValidForProcessing">
    <rdfs:domain rdf:resource="https://w3id.org/GConsent#Status"/>
    <rdfs:seeAlso xml:lang="en">The given consent renders the data as valid for processing by the current data controller. This data property was inspired by the "Status valid for Processing" class in GConsent.</rdfs:seeAlso>
    <rdfs:seeAlso>https://w3id.org/GConsent#StatusValidForProcessing</rdfs:seeAlso>
    <rdf:type rdf:resource="http://www.w3.org/2002/07/owl#DatatypeProperty"/>
    <rdfs:range rdf:resource="http://www.w3.org/2001/XMLSchema#boolean"/>
  </rdf:Description>
  <rdf:Description rdf:about="https://www.scss.tcd.ie/~kamarajk/EthicsOntology#hasPoliticalOpinions">
    <rdfs:comment xml:lang="en">Information about the data subject's political opinions are present.</rdfs:comment>
    <rdf:type rdf:resource="http://www.w3.org/2002/07/owl#DatatypeProperty"/>
    <rdfs:range rdf:resource="http://www.w3.org/2001/XMLSchema#boolean"/>
    <rdfs:domain rdf:resource="https://www.scss.tcd.ie/~kamarajk/EthicsOntology#Group"/>
    <rdfs:domain rdf:resource="https://www.scss.tcd.ie/~kamarajk/EthicsOntology#Individual"/>
  </rdf:Description>
  <rdf:Description rdf:about="https://www.scss.tcd.ie/~kamarajk/EthicsOntology#hasIncomeBracketData">
    <rdfs:domain rdf:resource="https://www.scss.tcd.ie/~kamarajk/EthicsOntology#Individual"/>
    <rdfs:domain rdf:resource="https://www.scss.tcd.ie/~kamarajk/EthicsOntology#Group"/>
    <rdfs:range rdf:resource="http://www.w3.org/2001/XMLSchema#boolean"/>
    <rdfs:seeAlso xml:lang="en">https://www.w3.org/ns/dpv#income-bracket</rdfs:seeAlso>
    <rdfs:comment xml:lang="en">Information about the data subject's income bracket is present. This data property was inspired by the "dpv:IncomeBracket" class in the Data Privacy Vocabulary (DPV).</rdfs:comment>
    <rdf:type rdf:resource="http://www.w3.org/2002/07/owl#DatatypeProperty"/>
  </rdf:Description>
  <rdf:Description rdf:about="https://www.scss.tcd.ie/~kamarajk/EthicsOntology#hasDateOfBirth">
    <rdfs:range rdf:resource="http://www.w3.org/2001/XMLSchema#boolean"/>
    <rdfs:domain rdf:resource="https://www.scss.tcd.ie/~kamarajk/EthicsOntology#Individual"/>
    <rdfs:comment xml:lang="en">Information about the data subject's date of birth is present.</rdfs:comment>
    <rdf:type rdf:resource="http://www.w3.org/2002/07/owl#DatatypeProperty"/>
  </rdf:Description>
  <rdf:Description rdf:about="https://www.scss.tcd.ie/~kamarajk/EthicsOntology#TestDataset">
    <isChild rdf:datatype="http://www.w3.org/2001/XMLSchema#boolean">false</isChild>
    <hasHealthData rdf:datatype="http://www.w3.org/2001/XMLSchema#boolean">false</hasHealthData>
    <hasEthnicityData rdf:datatype="http://www.w3.org/2001/XMLSchema#boolean">true</hasEthnicityData>
    <hasLoanRecords rdf:datatype="http://www.w3.org/2001/XMLSchema#boolean">false</hasLoanRecords>
    <hasName rdf:datatype="http://www.w3.org/2001/XMLSchema#boolean">true</hasName>
    <hasDoctorConsultationsData rdf:datatype="http://www.w3.org/2001/XMLSchema#boolean">false</hasDoctorConsultationsData>
    <hasUserTrackingData rdf:datatype="http://www.w3.org/2001/XMLSchema#boolean">true</hasUserTrackingData>
    <hasDataControllerName rdf:datatype="http://www.w3.org/2001/XMLSchema#boolean">false</hasDataControllerName>
    <hasContactInformation rdf:datatype="http://www.w3.org/2001/XMLSchema#boolean">true</hasContactInformation>
    <hasTooManyDataPoints rdf:datatype="http://www.w3.org/2001/XMLSchema#boolean">false</hasTooManyDataPoints>
    <hasIncomeData rdf:datatype="http://www.w3.org/2001/XMLSchema#boolean">true</hasIncomeData>
    <hasCriminalActivity rdf:datatype="http://www.w3.org/2001/XMLSchema#boolean">false</hasCriminalActivity>
    <hasBehaviourData rdf:datatype="http://www.w3.org/2001/XMLSchema#boolean">true</hasBehaviourData>
    <hasReligion rdf:datatype="http://www.w3.org/2001/XMLSchema#boolean">false</hasReligion>
    <hasAge rdf:datatype="http://www.w3.org/2001/XMLSchema#boolean">true</hasAge>
    <hasLocationData rdf:datatype="http://www.w3.org/2001/XMLSchema#boolean">false</hasLocationData>
    <hasSignedNDA rdf:datatype="http://www.w3.org/2001/XMLSchema#boolean">false</hasSignedNDA>
    <rdf:type rdf:resource="http://www.w3.org/2002/07/owl#NamedIndividual"/>
    <isValidForProcessing rdf:datatype="http://www.w3.org/2001/XMLSchema#boolean">false</isValidForProcessing>
    <hasPhysicalCharacteristics rdf:datatype="http://www.w3.org/2001/XMLSchema#boolean">true</hasPhysicalCharacteristics>
    <hasPoliticalOpinions rdf:datatype="http://www.w3.org/2001/XMLSchema#boolean">false</hasPoliticalOpinions>
    <hasBodyStatistics rdf:datatype="http://www.w3.org/2001/XMLSchema#boolean">false</hasBodyStatistics>
    <hasFilesWithPIIAttached rdf:datatype="http://www.w3.org/2001/XMLSchema#boolean">false</hasFilesWithPIIAttached>
  </rdf:Description>
  <rdf:Description rdf:about="https://www.scss.tcd.ie/~kamarajk/EthicsOntology#hasFilesWithPIIAttached">
    <rdfs:comment xml:lang="en">Files with the data subject's personally identifiable information (PII) is attached to the dataset. Example: Resume, photos, scanned financial documents, scanned doctor's report.</rdfs:comment>
    <rdf:type rdf:resource="http://www.w3.org/2002/07/owl#DatatypeProperty"/>
    <rdfs:domain rdf:resource="https://www.scss.tcd.ie/~kamarajk/EthicsOntology#Individual"/>
    <rdfs:range rdf:resource="http://www.w3.org/2001/XMLSchema#boolean"/>
  </rdf:Description>
  <rdf:Description rdf:about="https://www.scss.tcd.ie/~kamarajk/EthicsOntology#hasLocationData">
    <rdfs:seeAlso>https://www.w3.org/ns/dpv#dpv:Location</rdfs:seeAlso>
    <rdf:type rdf:resource="http://www.w3.org/2002/07/owl#DatatypeProperty"/>
    <rdfs:domain rdf:resource="https://www.scss.tcd.ie/~kamarajk/EthicsOntology#Individual"/>
    <rdfs:comment xml:lang="en">Information about the data subject's location is present. This data property was inspired by the "dpv:Location" class in the Data Privacy Vocabulary (DPV).</rdfs:comment>
    <rdfs:domain rdf:resource="https://www.scss.tcd.ie/~kamarajk/EthicsOntology#Group"/>
    <rdfs:range rdf:resource="http://www.w3.org/2001/XMLSchema#boolean"/>
  </rdf:Description>
  <rdf:Description rdf:about="https://www.scss.tcd.ie/~kamarajk/EthicsOntology#hasBehaviourData">
    <rdfs:domain rdf:resource="https://www.scss.tcd.ie/~kamarajk/EthicsOntology#Individual"/>
    <rdf:type rdf:resource="http://www.w3.org/2002/07/owl#DatatypeProperty"/>
    <rdfs:range rdf:resource="http://www.w3.org/2001/XMLSchema#boolean"/>
    <rdfs:comment xml:lang="en">Information about the data subject's behaviour is present. This data property was inspired by the "dpv:Behavioral" class in the Data Privacy Vocabulary (DPV).</rdfs:comment>
    <rdfs:seeAlso>https://www.w3.org/ns/dpv#dpv:Behavioral</rdfs:seeAlso>
  </rdf:Description>
  <rdf:Description rdf:about="https://www.scss.tcd.ie/~kamarajk/EthicsOntology#hasCriminalActivity">
    <rdfs:range rdf:resource="http://www.w3.org/2001/XMLSchema#boolean"/>
    <rdfs:seeAlso>https://www.w3.org/ns/dpv#criminal</rdfs:seeAlso>
    <rdfs:comment xml:lang="en">Information about the data subject's criminal activity is present. Example: criminal convictions or jail time. This data property was inspired by the "dpv:Criminal" class in the Data Privacy Vocabulary (DPV).</rdfs:comment>
    <rdf:type rdf:resource="http://www.w3.org/2002/07/owl#DatatypeProperty"/>
    <rdfs:domain rdf:resource="https://www.scss.tcd.ie/~kamarajk/EthicsOntology#Individual"/>
    <rdfs:domain rdf:resource="https://www.scss.tcd.ie/~kamarajk/EthicsOntology#Group"/>
  </rdf:Description>
  <rdf:Description rdf:about="https://www.scss.tcd.ie/~kamarajk/EthicsOntology#hasTooManyDataPoints">
    <rdfs:range rdf:resource="http://www.w3.org/2001/XMLSchema#boolean"/>
    <rdfs:domain rdf:resource="https://www.scss.tcd.ie/~kamarajk/EthicsOntology#Individual"/>
    <rdf:type rdf:resource="http://www.w3.org/2002/07/owl#DatatypeProperty"/>
    <rdfs:comment xml:lang="en">Too much of the data subject's data is present in the dataset.</rdfs:comment>
  </rdf:Description>
  <rdf:Description rdf:about="https://www.scss.tcd.ie/~kamarajk/EthicsOntology#Vocab_TestDataset">
    <isValidForProcessing rdf:datatype="http://www.w3.org/2001/XMLSchema#boolean">false</isValidForProcessing>
    <hasUserTrackingData rdf:datatype="http://www.w3.org/2001/XMLSchema#boolean">false</hasUserTrackingData>
    <rdf:type rdf:resource="http://www.w3.org/2002/07/owl#NamedIndividual"/>
    <hasEthnicityData rdf:datatype="http://www.w3.org/2001/XMLSchema#boolean">false</hasEthnicityData>
    <hasDataControllerName rdf:datatype="http://www.w3.org/2001/XMLSchema#boolean">false</hasDataControllerName>
    <hasCriminalActivity rdf:datatype="http://www.w3.org/2001/XMLSchema#boolean">false</hasCriminalActivity>
    <hasDoctorConsultationsData rdf:datatype="http://www.w3.org/2001/XMLSchema#boolean">false</hasDoctorConsultationsData>
    <hasPhysicalCharacteristics rdf:datatype="http://www.w3.org/2001/XMLSchema#boolean">false</hasPhysicalCharacteristics>
    <hasTooManyDataPoints rdf:datatype="http://www.w3.org/2001/XMLSchema#boolean">false</hasTooManyDataPoints>
    <hasFilesWithPIIAttached rdf:datatype="http://www.w3.org/2001/XMLSchema#boolean">false</hasFilesWithPIIAttached>
    <hasPoliticalOpinions rdf:datatype="http://www.w3.org/2001/XMLSchema#boolean">false</hasPoliticalOpinions>
    <hasIncomeData rdf:datatype="http://www.w3.org/2001/XMLSchema#boolean">false</hasIncomeData>
    <hasLocationData rdf:datatype="http://www.w3.org/2001/XMLSchema#boolean">true</hasLocationData>
    <hasAge rdf:datatype="http://www.w3.org/2001/XMLSchema#boolean">false</hasAge>
    <hasContactInformation rdf:datatype="http://www.w3.org/2001/XMLSchema#boolean">false</hasContactInformation>
    <hasSignedNDA rdf:datatype="http://www.w3.org/2001/XMLSchema#boolean">false</hasSignedNDA>
    <hasLoanRecords rdf:datatype="http://www.w3.org/2001/XMLSchema#boolean">false</hasLoanRecords>
    <isChild rdf:datatype="http://www.w3.org/2001/XMLSchema#boolean">false</isChild>
    <hasHealthData rdf:datatype="http://www.w3.org/2001/XMLSchema#boolean">false</hasHealthData>
    <hasBehaviourData rdf:datatype="http://www.w3.org/2001/XMLSchema#boolean">false</hasBehaviourData>
    <hasName rdf:datatype="http://www.w3.org/2001/XMLSchema#boolean">true</hasName>
    <hasBodyStatistics rdf:datatype="http://www.w3.org/2001/XMLSchema#boolean">false</hasBodyStatistics>
    <hasReligion rdf:datatype="http://www.w3.org/2001/XMLSchema#boolean">false</hasReligion>
  </rdf:Description>
  <rdf:Description rdf:about="https://www.scss.tcd.ie/~kamarajk/EthicsOntology#isStatusForConsent">
    <rdfs:domain rdf:resource="https://w3id.org/GConsent#Status"/>
    <rdfs:range rdf:resource="https://w3id.org/GConsent#Consent"/>
    <rdf:type rdf:resource="http://www.w3.org/2002/07/owl#ObjectProperty"/>
  </rdf:Description>
  <rdf:Description rdf:about="https://www.scss.tcd.ie/~kamarajk/EthicsOntology#hasDataControllerName">
    <rdfs:range rdf:resource="http://www.w3.org/2001/XMLSchema#string"/>
    <rdfs:domain rdf:resource="http://www.w3.org/ns/dpv#dpv:DataController"/>
    <rdfs:comment xml:lang="en">Indicates the name of the data controller.</rdfs:comment>
    <rdf:type rdf:resource="http://www.w3.org/2002/07/owl#DatatypeProperty"/>
  </rdf:Description>
  <rdf:Description rdf:about="https://www.scss.tcd.ie/~kamarajk/EthicsOntology#hasReligion">
    <rdfs:domain rdf:resource="https://www.scss.tcd.ie/~kamarajk/EthicsOntology#Group"/>
    <rdf:type rdf:resource="http://www.w3.org/2002/07/owl#DatatypeProperty"/>
    <rdfs:seeAlso>https://www.w3.org/ns/dpv#dpv:Religion</rdfs:seeAlso>
    <rdfs:comment xml:lang="en">Information about the data subject's religion, religious inclinations, and religious history is present. This data property was inspired by the "dpv:Religion" class in the Data Privacy Vocabulary (DPV).</rdfs:comment>
    <rdfs:domain rdf:resource="https://www.scss.tcd.ie/~kamarajk/EthicsOntology#Individual"/>
    <rdfs:range rdf:resource="http://www.w3.org/2001/XMLSchema#boolean"/>
  </rdf:Description>
  <rdf:Description rdf:about="https://www.scss.tcd.ie/~kamarajk/EthicsOntology#hasUserTrackingData">
    <rdfs:domain rdf:resource="https://www.scss.tcd.ie/~kamarajk/EthicsOntology#Individual"/>
    <rdf:type rdf:resource="http://www.w3.org/2002/07/owl#DatatypeProperty"/>
    <rdfs:comment xml:lang="en">Data that is related to tracking the data subject (online or offline) is present. This data property was inspired by the "dpv:Tracking" class in the Data Privacy Vocabulary (DPV).</rdfs:comment>
    <rdfs:seeAlso>https://www.w3.org/ns/dpv#dpv:Tracking</rdfs:seeAlso>
    <rdfs:range rdf:resource="http://www.w3.org/2001/XMLSchema#boolean"/>
    <rdfs:domain rdf:resource="https://www.scss.tcd.ie/~kamarajk/EthicsOntology#Group"/>
  </rdf:Description>
  <rdf:Description rdf:about="https://w3id.org/GConsent#hasConsent">
    <rdfs:domain rdf:resource="http://www.w3.org/ns/dpv#dpv:DataSubject"/>
    <rdfs:range rdf:resource="https://w3id.org/GConsent#Consent"/>
    <rdf:type rdf:resource="http://www.w3.org/2002/07/owl#ObjectProperty"/>
    <owl:inverseOf rdf:resource="https://w3id.org/GConsent#isConsentForDataSubject"/>
  </rdf:Description>
  <rdf:Description rdf:about="https://w3id.org/GConsent#isConsentForDataSubject">
    <rdfs:domain rdf:resource="https://w3id.org/GConsent#Consent"/>
    <rdfs:range rdf:resource="http://www.w3.org/ns/dpv#dpv:DataSubject"/>
    <rdf:type rdf:resource="http://www.w3.org/2002/07/owl#ObjectProperty"/>
  </rdf:Description>
  <rdf:Description rdf:about="http://www.w3.org/ns/dpv#dpv:DataController">
    <rdf:type rdf:resource="http://www.w3.org/2002/07/owl#Class"/>
    <rdfs:label xml:lang="en">Data Controller</rdfs:label>
  </rdf:Description>
  <rdf:Description rdf:about="https://www.scss.tcd.ie/~kamarajk/EthicsOntology#hasStatus">
    <rdf:type rdf:resource="http://www.w3.org/2002/07/owl#ObjectProperty"/>
    <rdfs:domain rdf:resource="https://w3id.org/GConsent#Consent"/>
    <owl:inverseOf rdf:resource="https://www.scss.tcd.ie/~kamarajk/EthicsOntology#isStatusForConsent"/>
    <rdfs:range rdf:resource="https://w3id.org/GConsent#Status"/>
  </rdf:Description>
  <rdf:Description rdf:about="http://www.w3.org/ns/dpv#dpv:DataSubject">
    <rdfs:label xml:lang="en">Data Subject</rdfs:label>
    <rdf:type rdf:resource="http://www.w3.org/2002/07/owl#Class"/>
  </rdf:Description>
  <rdf:Description rdf:about="https://www.scss.tcd.ie/~kamarajk/EthicsOntology#hasContactInformation">
    <rdf:type rdf:resource="http://www.w3.org/2002/07/owl#DatatypeProperty"/>
    <rdfs:comment xml:lang="en">Information about the data subject's contact details is present. Example: telephone number or email address. This data property was inspired by the "dpv:Contact" class in the Data Privacy Vocabulary (DPV).</rdfs:comment>
    <rdfs:domain rdf:resource="https://www.scss.tcd.ie/~kamarajk/EthicsOntology#Individual"/>
    <rdfs:seeAlso>https://www.w3.org/ns/dpv#dpv:Contact</rdfs:seeAlso>
    <rdfs:range rdf:resource="http://www.w3.org/2001/XMLSchema#boolean"/>
  </rdf:Description>
  <rdf:Description rdf:about="https://www.scss.tcd.ie/~kamarajk/EthicsOntology#hasDoctorConsultationsData">
    <rdfs:comment xml:lang="en">Information about the data subject's doctor consultations is present.</rdfs:comment>
    <rdf:type rdf:resource="http://www.w3.org/2002/07/owl#DatatypeProperty"/>
    <rdfs:range rdf:resource="http://www.w3.org/2001/XMLSchema#boolean"/>
    <rdfs:domain rdf:resource="https://www.scss.tcd.ie/~kamarajk/EthicsOntology#Group"/>
    <rdfs:domain rdf:resource="https://www.scss.tcd.ie/~kamarajk/EthicsOntology#Individual"/>
  </rdf:Description>
  <rdf:Description rdf:about="https://www.scss.tcd.ie/~kamarajk/EthicsOntology#hasSexualData">
    <rdf:type rdf:resource="http://www.w3.org/2002/07/owl#DatatypeProperty"/>
    <rdfs:seeAlso>https://www.w3.org/ns/dpv#dpv:Sexual</rdfs:seeAlso>
    <rdfs:range rdf:resource="http://www.w3.org/2001/XMLSchema#boolean"/>
    <rdfs:domain rdf:resource="https://www.scss.tcd.ie/~kamarajk/EthicsOntology#Group"/>
    <rdfs:comment xml:lang="en">Information that describes the data subject's sexual life is present. This data property was inspired by the "dpv:Sexual" class in the Data Privacy Vocabulary (DPV).</rdfs:comment>
    <rdfs:domain rdf:resource="https://www.scss.tcd.ie/~kamarajk/EthicsOntology#Individual"/>
  </rdf:Description>
  <rdf:Description rdf:about="https://www.scss.tcd.ie/~kamarajk/EthicsOntology#hasAge">
    <rdfs:range rdf:resource="http://www.w3.org/2001/XMLSchema#boolean"/>
    <rdf:type rdf:resource="http://www.w3.org/2002/07/owl#DatatypeProperty"/>
    <rdfs:seeAlso>https://www.w3.org/ns/dpv#dpv:Age</rdfs:seeAlso>
    <rdfs:domain rdf:resource="https://www.scss.tcd.ie/~kamarajk/EthicsOntology#Individual"/>
    <rdfs:comment xml:lang="en">Information about the data subjectâ€™s age is present. This data property was inspired by the "dpv:Age" class in the Data Privacy Vocabulary (DPV).</rdfs:comment>
    <rdfs:domain rdf:resource="https://www.scss.tcd.ie/~kamarajk/EthicsOntology#Group"/>
  </rdf:Description>
  <rdf:Description rdf:about="https://www.scss.tcd.ie/~kamarajk/EthicsOntology#hasName">
    <rdfs:seeAlso>https://www.w3.org/ns/dpv#dpv:Name</rdfs:seeAlso>
    <rdf:type rdf:resource="http://www.w3.org/2002/07/owl#DatatypeProperty"/>
    <rdfs:range rdf:resource="http://www.w3.org/2001/XMLSchema#boolean"/>
    <rdfs:comment xml:lang="en">Information about the data subject's name is present. This data property was inspired by the "dpv:Name" class in the Data Privacy Vocabulary (DPV).

In some cases, an individual's name can be used to identify the caste, race, religion, or country the individual belongs too.</rdfs:comment>
    <rdfs:domain rdf:resource="https://www.scss.tcd.ie/~kamarajk/EthicsOntology#Individual"/>
  </rdf:Description>
  <rdf:Description rdf:about="https://www.scss.tcd.ie/~kamarajk/EthicsOntology#hasPhysicalCharacteristics">
    <rdfs:seeAlso>https://www.w3.org/ns/dpv#dpv:PhysicalCharacteristic</rdfs:seeAlso>
    <rdfs:domain rdf:resource="https://www.scss.tcd.ie/~kamarajk/EthicsOntology#Group"/>
    <rdfs:range rdf:resource="http://www.w3.org/2001/XMLSchema#boolean"/>
    <rdf:type rdf:resource="http://www.w3.org/2002/07/owl#DatatypeProperty"/>
    <rdfs:comment xml:lang="en">Information about the data subject's physical characteristics is present. Example: gender, physical disabilities, skin colour, hair colour, tattoos, piercings. This data property was inspired by the "dpv:PhysicalCharacteristic" class in the Data Privacy Vocabulary (DPV).</rdfs:comment>
    <rdfs:domain rdf:resource="https://www.scss.tcd.ie/~kamarajk/EthicsOntology#Individual"/>
  </rdf:Description>
  <rdf:Description rdf:about="https://www.scss.tcd.ie/~kamarajk/EthicsOntology#hasSignedNDA">
    <rdfs:comment xml:lang="en">Information about any Non-disclosure agreements (NDA) that the data subject may have signed is present. This data property was inspired by the "dpv:NDA" class in the Data Privacy Vocabulary (DPV).</rdfs:comment>
    <rdf:type rdf:resource="http://www.w3.org/2002/07/owl#DatatypeProperty"/>
    <rdfs:seeAlso>https://www.w3.org/ns/dpv#dpv:NDA</rdfs:seeAlso>
    <rdfs:domain rdf:resource="https://www.scss.tcd.ie/~kamarajk/EthicsOntology#Individual"/>
    <rdfs:range rdf:resource="http://www.w3.org/2001/XMLSchema#boolean"/>
  </rdf:Description>
  <rdf:Description rdf:about="https://w3id.org/GConsent#isProvidedToController">
    <rdfs:domain rdf:resource="https://w3id.org/GConsent#Consent"/>
    <owl:inverseOf rdf:resource="https://w3id.org/GConsent#wasProvidedConsent"/>
    <rdf:type rdf:resource="http://www.w3.org/2002/07/owl#ObjectProperty"/>
    <rdfs:range rdf:resource="http://www.w3.org/ns/dpv#dpv:DataController"/>
    <rdf:type rdf:resource="http://www.w3.org/2002/07/owl#IrreflexiveProperty"/>
    <rdf:type rdf:resource="http://www.w3.org/2002/07/owl#InverseFunctionalProperty"/>
    <rdf:type rdf:resource="http://www.w3.org/2002/07/owl#AsymmetricProperty"/>
  </rdf:Description>
  <rdf:Description rdf:about="https://www.scss.tcd.ie/~kamarajk/EthicsOntology#Individual">
    <rdfs:subClassOf rdf:resource="http://www.w3.org/ns/dpv#dpv:DataSubject"/>
    <rdfs:comment xml:lang="en">Describes the data subject when it is an individual, that is when the dataset represents specific people.</rdfs:comment>
    <rdf:type rdf:resource="http://www.w3.org/2002/07/owl#Class"/>
  </rdf:Description>
  <rdf:Description rdf:about="https://w3id.org/GConsent#wasProvidedConsent">
    <rdfs:domain rdf:resource="http://www.w3.org/ns/dpv#dpv:DataController"/>
    <rdfs:range rdf:resource="https://w3id.org/GConsent#Consent"/>
    <rdf:type rdf:resource="http://www.w3.org/2002/07/owl#ObjectProperty"/>
  </rdf:Description>
  <rdf:Description rdf:about="https://www.scss.tcd.ie/~kamarajk/EthicsOntology#hasBodyStatistics">
    <rdfs:range rdf:resource="http://www.w3.org/2001/XMLSchema#boolean"/>
    <rdfs:domain rdf:resource="https://www.scss.tcd.ie/~kamarajk/EthicsOntology#Group"/>
    <rdf:type rdf:resource="http://www.w3.org/2002/07/owl#DatatypeProperty"/>
    <rdfs:domain rdf:resource="https://www.scss.tcd.ie/~kamarajk/EthicsOntology#Individual"/>
    <rdfs:comment xml:lang="en">Information about the data subject's physical metrics such as height, weight, waist size is present.</rdfs:comment>
  </rdf:Description>
  <rdf:Description rdf:about="https://www.scss.tcd.ie/~kamarajk/EthicsOntology#Group">
    <rdfs:comment xml:lang="en">Describes the data subject when it is a group, that is when the dataset represents different races, religions, or people with a certain disability.</rdfs:comment>
    <owl:disjointWith rdf:resource="https://www.scss.tcd.ie/~kamarajk/EthicsOntology#Individual"/>
    <rdf:type rdf:resource="http://www.w3.org/2002/07/owl#Class"/>
    <rdfs:subClassOf rdf:resource="http://www.w3.org/ns/dpv#dpv:DataSubject"/>
  </rdf:Description>
  <rdf:Description rdf:about="https://w3id.org/GConsent#Status">
    <rdf:type rdf:resource="http://www.w3.org/2002/07/owl#Class"/>
  </rdf:Description>
  <rdf:Description rdf:about="https://www.scss.tcd.ie/~kamarajk/EthicsOntology#hasLoanRecords">
    <rdfs:comment xml:lang="en">Information about the loans provided to the the data subject or other related information is present. This data property was inspired by the "dpv:LoanRecord" class in the Data Privacy Vocabulary (DPV).</rdfs:comment>
    <rdfs:domain rdf:resource="https://www.scss.tcd.ie/~kamarajk/EthicsOntology#Group"/>
    <rdfs:seeAlso>https://www.w3.org/ns/dpv#dpv:LoanRecord</rdfs:seeAlso>
    <rdfs:domain rdf:resource="https://www.scss.tcd.ie/~kamarajk/EthicsOntology#Individual"/>
    <rdf:type rdf:resource="http://www.w3.org/2002/07/owl#DatatypeProperty"/>
    <rdfs:range rdf:resource="http://www.w3.org/2001/XMLSchema#boolean"/>
  </rdf:Description>
  <rdf:Description rdf:about="https://w3id.org/GConsent#Consent">
    <rdf:type rdf:resource="http://www.w3.org/2002/07/owl#Class"/>
  </rdf:Description>
  <rdf:Description rdf:about="https://www.scss.tcd.ie/~kamarajk/EthicsOntology">
    <rdf:type rdf:resource="http://www.w3.org/2002/07/owl#Ontology"/>
  </rdf:Description>
</rdf:RDF>
