<?xml version="1.0"?>
<rdf:RDF xmlns="https://www.scss.tcd.ie/~kamarajk/EthicsOntology#"
     xml:base="https://www.scss.tcd.ie/~kamarajk/EthicsOntology"
     xmlns:owl="http://www.w3.org/2002/07/owl#"
     xmlns:rdf="http://www.w3.org/1999/02/22-rdf-syntax-ns#"
     xmlns:xml="http://www.w3.org/XML/1998/namespace"
     xmlns:xsd="http://www.w3.org/2001/XMLSchema#"
     xmlns:rdfs="http://www.w3.org/2000/01/rdf-schema#">
    <owl:Ontology rdf:about="https://www.scss.tcd.ie/~kamarajk/EthicsOntology"/>
    


    <!-- 
    ///////////////////////////////////////////////////////////////////////////////////////
    //
    // Object Properties
    //
    ///////////////////////////////////////////////////////////////////////////////////////
     -->

    


    <!-- https://w3id.org/GConsent#hasConsent -->

    <owl:ObjectProperty rdf:about="https://w3id.org/GConsent#hasConsent">
        <owl:inverseOf rdf:resource="https://w3id.org/GConsent#isConsentForDataSubject"/>
        <rdfs:domain rdf:resource="http://www.w3.org/ns/dpv#dpv:DataSubject"/>
        <rdfs:range rdf:resource="https://w3id.org/GConsent#Consent"/>
    </owl:ObjectProperty>
    


    <!-- https://w3id.org/GConsent#isConsentForDataSubject -->

    <owl:ObjectProperty rdf:about="https://w3id.org/GConsent#isConsentForDataSubject">
        <rdfs:domain rdf:resource="https://w3id.org/GConsent#Consent"/>
        <rdfs:range rdf:resource="http://www.w3.org/ns/dpv#dpv:DataSubject"/>
    </owl:ObjectProperty>
    


    <!-- https://w3id.org/GConsent#isProvidedToController -->

    <owl:ObjectProperty rdf:about="https://w3id.org/GConsent#isProvidedToController">
        <owl:inverseOf rdf:resource="https://w3id.org/GConsent#wasProvidedConsent"/>
        <rdf:type rdf:resource="http://www.w3.org/2002/07/owl#InverseFunctionalProperty"/>
        <rdf:type rdf:resource="http://www.w3.org/2002/07/owl#AsymmetricProperty"/>
        <rdf:type rdf:resource="http://www.w3.org/2002/07/owl#IrreflexiveProperty"/>
        <rdfs:domain rdf:resource="https://w3id.org/GConsent#Consent"/>
        <rdfs:range rdf:resource="http://www.w3.org/ns/dpv#dpv:DataController"/>
    </owl:ObjectProperty>
    


    <!-- https://w3id.org/GConsent#wasProvidedConsent -->

    <owl:ObjectProperty rdf:about="https://w3id.org/GConsent#wasProvidedConsent">
        <rdfs:domain rdf:resource="http://www.w3.org/ns/dpv#dpv:DataController"/>
        <rdfs:range rdf:resource="https://w3id.org/GConsent#Consent"/>
    </owl:ObjectProperty>
    


    <!-- https://www.scss.tcd.ie/~kamarajk/EthicsOntology#hasStatus -->

    <owl:ObjectProperty rdf:about="https://www.scss.tcd.ie/~kamarajk/EthicsOntology#hasStatus">
        <owl:inverseOf rdf:resource="https://www.scss.tcd.ie/~kamarajk/EthicsOntology#isStatusForConsent"/>
        <rdfs:domain rdf:resource="https://w3id.org/GConsent#Consent"/>
        <rdfs:range rdf:resource="https://w3id.org/GConsent#Status"/>
    </owl:ObjectProperty>
    


    <!-- https://www.scss.tcd.ie/~kamarajk/EthicsOntology#isStatusForConsent -->

    <owl:ObjectProperty rdf:about="https://www.scss.tcd.ie/~kamarajk/EthicsOntology#isStatusForConsent">
        <rdfs:domain rdf:resource="https://w3id.org/GConsent#Status"/>
        <rdfs:range rdf:resource="https://w3id.org/GConsent#Consent"/>
    </owl:ObjectProperty>
    


    <!-- 
    ///////////////////////////////////////////////////////////////////////////////////////
    //
    // Data properties
    //
    ///////////////////////////////////////////////////////////////////////////////////////
     -->

    


    <!-- https://www.scss.tcd.ie/~kamarajk/EthicsOntology#hasAge -->

    <owl:DatatypeProperty rdf:about="https://www.scss.tcd.ie/~kamarajk/EthicsOntology#hasAge">
        <rdfs:domain rdf:resource="https://www.scss.tcd.ie/~kamarajk/EthicsOntology#Group"/>
        <rdfs:domain rdf:resource="https://www.scss.tcd.ie/~kamarajk/EthicsOntology#Individual"/>
        <rdfs:range rdf:resource="http://www.w3.org/2001/XMLSchema#boolean"/>
        <rdfs:comment xml:lang="en">Information about the data subject’s age is present. This data property was inspired by the &quot;dpv:Age&quot; class in the Data Privacy Vocabulary (DPV).</rdfs:comment>
        <rdfs:seeAlso>https://www.w3.org/ns/dpv#dpv:Age</rdfs:seeAlso>
    </owl:DatatypeProperty>
    


    <!-- https://www.scss.tcd.ie/~kamarajk/EthicsOntology#hasBehaviourData -->

    <owl:DatatypeProperty rdf:about="https://www.scss.tcd.ie/~kamarajk/EthicsOntology#hasBehaviourData">
        <rdfs:domain rdf:resource="https://www.scss.tcd.ie/~kamarajk/EthicsOntology#Individual"/>
        <rdfs:range rdf:resource="http://www.w3.org/2001/XMLSchema#boolean"/>
        <rdfs:comment xml:lang="en">Information about the data subject&apos;s behaviour is present. This data property was inspired by the &quot;dpv:Behavioral&quot; class in the Data Privacy Vocabulary (DPV).</rdfs:comment>
        <rdfs:seeAlso>https://www.w3.org/ns/dpv#dpv:Behavioral</rdfs:seeAlso>
    </owl:DatatypeProperty>
    


    <!-- https://www.scss.tcd.ie/~kamarajk/EthicsOntology#hasBodyStatistics -->

    <owl:DatatypeProperty rdf:about="https://www.scss.tcd.ie/~kamarajk/EthicsOntology#hasBodyStatistics">
        <rdfs:domain rdf:resource="https://www.scss.tcd.ie/~kamarajk/EthicsOntology#Group"/>
        <rdfs:domain rdf:resource="https://www.scss.tcd.ie/~kamarajk/EthicsOntology#Individual"/>
        <rdfs:range rdf:resource="http://www.w3.org/2001/XMLSchema#boolean"/>
        <rdfs:comment xml:lang="en">Information about the data subject&apos;s physical metrics such as height, weight, waist size is present.</rdfs:comment>
    </owl:DatatypeProperty>
    


    <!-- https://www.scss.tcd.ie/~kamarajk/EthicsOntology#hasContactInformation -->

    <owl:DatatypeProperty rdf:about="https://www.scss.tcd.ie/~kamarajk/EthicsOntology#hasContactInformation">
        <rdfs:domain rdf:resource="https://www.scss.tcd.ie/~kamarajk/EthicsOntology#Individual"/>
        <rdfs:range rdf:resource="http://www.w3.org/2001/XMLSchema#boolean"/>
        <rdfs:comment xml:lang="en">Information about the data subject&apos;s contact details is present. Example: telephone number or email address. This data property was inspired by the &quot;dpv:Contact&quot; class in the Data Privacy Vocabulary (DPV).</rdfs:comment>
        <rdfs:seeAlso>https://www.w3.org/ns/dpv#dpv:Contact</rdfs:seeAlso>
    </owl:DatatypeProperty>
    


    <!-- https://www.scss.tcd.ie/~kamarajk/EthicsOntology#hasCriminalActivity -->

    <owl:DatatypeProperty rdf:about="https://www.scss.tcd.ie/~kamarajk/EthicsOntology#hasCriminalActivity">
        <rdfs:domain rdf:resource="https://www.scss.tcd.ie/~kamarajk/EthicsOntology#Group"/>
        <rdfs:domain rdf:resource="https://www.scss.tcd.ie/~kamarajk/EthicsOntology#Individual"/>
        <rdfs:range rdf:resource="http://www.w3.org/2001/XMLSchema#boolean"/>
        <rdfs:comment xml:lang="en">Information about the data subject&apos;s criminal activity is present. Example: criminal convictions or jail time. This data property was inspired by the &quot;dpv:Criminal&quot; class in the Data Privacy Vocabulary (DPV).</rdfs:comment>
        <rdfs:seeAlso>https://www.w3.org/ns/dpv#criminal</rdfs:seeAlso>
    </owl:DatatypeProperty>
    


    <!-- https://www.scss.tcd.ie/~kamarajk/EthicsOntology#hasDataControllerName -->

    <owl:DatatypeProperty rdf:about="https://www.scss.tcd.ie/~kamarajk/EthicsOntology#hasDataControllerName">
        <rdfs:domain rdf:resource="http://www.w3.org/ns/dpv#dpv:DataController"/>
        <rdfs:range rdf:resource="http://www.w3.org/2001/XMLSchema#string"/>
        <rdfs:comment xml:lang="en">Indicates the name of the data controller.</rdfs:comment>
    </owl:DatatypeProperty>
    


    <!-- https://www.scss.tcd.ie/~kamarajk/EthicsOntology#hasDateOfBirth -->

    <owl:DatatypeProperty rdf:about="https://www.scss.tcd.ie/~kamarajk/EthicsOntology#hasDateOfBirth">
        <rdfs:domain rdf:resource="https://www.scss.tcd.ie/~kamarajk/EthicsOntology#Individual"/>
        <rdfs:range rdf:resource="http://www.w3.org/2001/XMLSchema#boolean"/>
        <rdfs:comment xml:lang="en">Information about the data subject&apos;s date of birth is present.</rdfs:comment>
    </owl:DatatypeProperty>
    


    <!-- https://www.scss.tcd.ie/~kamarajk/EthicsOntology#hasDoctorConsultationsData -->

    <owl:DatatypeProperty rdf:about="https://www.scss.tcd.ie/~kamarajk/EthicsOntology#hasDoctorConsultationsData">
        <rdfs:domain rdf:resource="https://www.scss.tcd.ie/~kamarajk/EthicsOntology#Group"/>
        <rdfs:domain rdf:resource="https://www.scss.tcd.ie/~kamarajk/EthicsOntology#Individual"/>
        <rdfs:range rdf:resource="http://www.w3.org/2001/XMLSchema#boolean"/>
        <rdfs:comment xml:lang="en">Information about the data subject&apos;s doctor consultations is present.</rdfs:comment>
    </owl:DatatypeProperty>
    


    <!-- https://www.scss.tcd.ie/~kamarajk/EthicsOntology#hasEthnicityData -->

    <owl:DatatypeProperty rdf:about="https://www.scss.tcd.ie/~kamarajk/EthicsOntology#hasEthnicityData">
        <rdfs:domain rdf:resource="https://www.scss.tcd.ie/~kamarajk/EthicsOntology#Group"/>
        <rdfs:domain rdf:resource="https://www.scss.tcd.ie/~kamarajk/EthicsOntology#Individual"/>
        <rdfs:range rdf:resource="http://www.w3.org/2001/XMLSchema#boolean"/>
        <rdfs:comment xml:lang="en">Information about the data subject’s origins and lineage is present. This data property was inspired by the &quot;dpv:Ethnicity&quot; class in the Data Privacy Vocabulary (DPV).

Ethicity data is any data that involves the data subject&apos;s ethnic origin, native language, race, caste, accent, dialect, or the immigration status of the data subject or their parents.</rdfs:comment>
        <rdfs:seeAlso>https://www.w3.org/ns/dpv#dpv:Ethnicity</rdfs:seeAlso>
    </owl:DatatypeProperty>
    


    <!-- https://www.scss.tcd.ie/~kamarajk/EthicsOntology#hasFilesWithPIIAttached -->

    <owl:DatatypeProperty rdf:about="https://www.scss.tcd.ie/~kamarajk/EthicsOntology#hasFilesWithPIIAttached">
        <rdfs:domain rdf:resource="https://www.scss.tcd.ie/~kamarajk/EthicsOntology#Individual"/>
        <rdfs:range rdf:resource="http://www.w3.org/2001/XMLSchema#boolean"/>
        <rdfs:comment xml:lang="en">Files with the data subject&apos;s personally identifiable information (PII) is attached to the dataset. Example: Resume, photos, scanned financial documents, scanned doctor&apos;s report.</rdfs:comment>
    </owl:DatatypeProperty>
    


    <!-- https://www.scss.tcd.ie/~kamarajk/EthicsOntology#hasHealthData -->

    <owl:DatatypeProperty rdf:about="https://www.scss.tcd.ie/~kamarajk/EthicsOntology#hasHealthData">
        <rdfs:domain rdf:resource="https://www.scss.tcd.ie/~kamarajk/EthicsOntology#Group"/>
        <rdfs:domain rdf:resource="https://www.scss.tcd.ie/~kamarajk/EthicsOntology#Individual"/>
        <rdfs:range rdf:resource="http://www.w3.org/2001/XMLSchema#boolean"/>
        <rdfs:comment xml:lang="en">Information about the data subject&apos;s health, medical conditions or health care (medical history, test results, etc.) is present. This data property was inspired by the &quot;dpv:MedicalHealth&quot; class in the Data Privacy Vocabulary (DPV).</rdfs:comment>
        <rdfs:seeAlso>https://www.w3.org/ns/dpv#dpv:MedicalHealth</rdfs:seeAlso>
    </owl:DatatypeProperty>
    


    <!-- https://www.scss.tcd.ie/~kamarajk/EthicsOntology#hasIncomeBracketData -->

    <owl:DatatypeProperty rdf:about="https://www.scss.tcd.ie/~kamarajk/EthicsOntology#hasIncomeBracketData">
        <rdfs:domain rdf:resource="https://www.scss.tcd.ie/~kamarajk/EthicsOntology#Group"/>
        <rdfs:domain rdf:resource="https://www.scss.tcd.ie/~kamarajk/EthicsOntology#Individual"/>
        <rdfs:range rdf:resource="http://www.w3.org/2001/XMLSchema#boolean"/>
        <rdfs:comment xml:lang="en">Information about the data subject&apos;s income bracket is present. This data property was inspired by the &quot;dpv:IncomeBracket&quot; class in the Data Privacy Vocabulary (DPV).</rdfs:comment>
        <rdfs:seeAlso xml:lang="en">https://www.w3.org/ns/dpv#income-bracket</rdfs:seeAlso>
    </owl:DatatypeProperty>
    


    <!-- https://www.scss.tcd.ie/~kamarajk/EthicsOntology#hasIncomeData -->

    <owl:DatatypeProperty rdf:about="https://www.scss.tcd.ie/~kamarajk/EthicsOntology#hasIncomeData">
        <rdfs:domain rdf:resource="https://www.scss.tcd.ie/~kamarajk/EthicsOntology#Individual"/>
        <rdfs:range rdf:resource="http://www.w3.org/2001/XMLSchema#boolean"/>
        <rdfs:comment xml:lang="en">Information about the data subject&apos;s income is present. This data property was inspired by the &quot;dpv:Income&quot; class in the Data Privacy Vocabulary (DPV).</rdfs:comment>
        <rdfs:seeAlso>https://www.w3.org/ns/dpv#income</rdfs:seeAlso>
    </owl:DatatypeProperty>
    


    <!-- https://www.scss.tcd.ie/~kamarajk/EthicsOntology#hasLoanRecords -->

    <owl:DatatypeProperty rdf:about="https://www.scss.tcd.ie/~kamarajk/EthicsOntology#hasLoanRecords">
        <rdfs:domain rdf:resource="https://www.scss.tcd.ie/~kamarajk/EthicsOntology#Group"/>
        <rdfs:domain rdf:resource="https://www.scss.tcd.ie/~kamarajk/EthicsOntology#Individual"/>
        <rdfs:range rdf:resource="http://www.w3.org/2001/XMLSchema#boolean"/>
        <rdfs:comment xml:lang="en">Information about the loans provided to the the data subject or other related information is present. This data property was inspired by the &quot;dpv:LoanRecord&quot; class in the Data Privacy Vocabulary (DPV).</rdfs:comment>
        <rdfs:seeAlso>https://www.w3.org/ns/dpv#dpv:LoanRecord</rdfs:seeAlso>
    </owl:DatatypeProperty>
    


    <!-- https://www.scss.tcd.ie/~kamarajk/EthicsOntology#hasLocationData -->

    <owl:DatatypeProperty rdf:about="https://www.scss.tcd.ie/~kamarajk/EthicsOntology#hasLocationData">
        <rdfs:domain rdf:resource="https://www.scss.tcd.ie/~kamarajk/EthicsOntology#Group"/>
        <rdfs:domain rdf:resource="https://www.scss.tcd.ie/~kamarajk/EthicsOntology#Individual"/>
        <rdfs:range rdf:resource="http://www.w3.org/2001/XMLSchema#boolean"/>
        <rdfs:comment xml:lang="en">Information about the data subject&apos;s location is present. This data property was inspired by the &quot;dpv:Location&quot; class in the Data Privacy Vocabulary (DPV).</rdfs:comment>
        <rdfs:seeAlso>https://www.w3.org/ns/dpv#dpv:Location</rdfs:seeAlso>
    </owl:DatatypeProperty>
    


    <!-- https://www.scss.tcd.ie/~kamarajk/EthicsOntology#hasName -->

    <owl:DatatypeProperty rdf:about="https://www.scss.tcd.ie/~kamarajk/EthicsOntology#hasName">
        <rdfs:domain rdf:resource="https://www.scss.tcd.ie/~kamarajk/EthicsOntology#Individual"/>
        <rdfs:range rdf:resource="http://www.w3.org/2001/XMLSchema#boolean"/>
        <rdfs:comment xml:lang="en">Information about the data subject&apos;s name is present. This data property was inspired by the &quot;dpv:Name&quot; class in the Data Privacy Vocabulary (DPV).

In some cases, an individual&apos;s name can be used to identify the caste, race, religion, or country the individual belongs too.</rdfs:comment>
        <rdfs:seeAlso>https://www.w3.org/ns/dpv#dpv:Name</rdfs:seeAlso>
    </owl:DatatypeProperty>
    


    <!-- https://www.scss.tcd.ie/~kamarajk/EthicsOntology#hasPhysicalCharacteristics -->

    <owl:DatatypeProperty rdf:about="https://www.scss.tcd.ie/~kamarajk/EthicsOntology#hasPhysicalCharacteristics">
        <rdfs:domain rdf:resource="https://www.scss.tcd.ie/~kamarajk/EthicsOntology#Group"/>
        <rdfs:domain rdf:resource="https://www.scss.tcd.ie/~kamarajk/EthicsOntology#Individual"/>
        <rdfs:range rdf:resource="http://www.w3.org/2001/XMLSchema#boolean"/>
        <rdfs:comment xml:lang="en">Information about the data subject&apos;s physical characteristics is present. Example: gender, physical disabilities, skin colour, hair colour, tattoos, piercings. This data property was inspired by the &quot;dpv:PhysicalCharacteristic&quot; class in the Data Privacy Vocabulary (DPV).</rdfs:comment>
        <rdfs:seeAlso>https://www.w3.org/ns/dpv#dpv:PhysicalCharacteristic</rdfs:seeAlso>
    </owl:DatatypeProperty>
    


    <!-- https://www.scss.tcd.ie/~kamarajk/EthicsOntology#hasPoliticalOpinions -->

    <owl:DatatypeProperty rdf:about="https://www.scss.tcd.ie/~kamarajk/EthicsOntology#hasPoliticalOpinions">
        <rdfs:domain rdf:resource="https://www.scss.tcd.ie/~kamarajk/EthicsOntology#Group"/>
        <rdfs:domain rdf:resource="https://www.scss.tcd.ie/~kamarajk/EthicsOntology#Individual"/>
        <rdfs:range rdf:resource="http://www.w3.org/2001/XMLSchema#boolean"/>
        <rdfs:comment xml:lang="en">Information about the data subject&apos;s political opinions are present.</rdfs:comment>
    </owl:DatatypeProperty>
    


    <!-- https://www.scss.tcd.ie/~kamarajk/EthicsOntology#hasReligion -->

    <owl:DatatypeProperty rdf:about="https://www.scss.tcd.ie/~kamarajk/EthicsOntology#hasReligion">
        <rdfs:domain rdf:resource="https://www.scss.tcd.ie/~kamarajk/EthicsOntology#Group"/>
        <rdfs:domain rdf:resource="https://www.scss.tcd.ie/~kamarajk/EthicsOntology#Individual"/>
        <rdfs:range rdf:resource="http://www.w3.org/2001/XMLSchema#boolean"/>
        <rdfs:comment xml:lang="en">Information about the data subject&apos;s religion, religious inclinations, and religious history is present. This data property was inspired by the &quot;dpv:Religion&quot; class in the Data Privacy Vocabulary (DPV).</rdfs:comment>
        <rdfs:seeAlso>https://www.w3.org/ns/dpv#dpv:Religion</rdfs:seeAlso>
    </owl:DatatypeProperty>
    


    <!-- https://www.scss.tcd.ie/~kamarajk/EthicsOntology#hasSexualData -->

    <owl:DatatypeProperty rdf:about="https://www.scss.tcd.ie/~kamarajk/EthicsOntology#hasSexualData">
        <rdfs:domain rdf:resource="https://www.scss.tcd.ie/~kamarajk/EthicsOntology#Group"/>
        <rdfs:domain rdf:resource="https://www.scss.tcd.ie/~kamarajk/EthicsOntology#Individual"/>
        <rdfs:range rdf:resource="http://www.w3.org/2001/XMLSchema#boolean"/>
        <rdfs:comment xml:lang="en">Information that describes the data subject&apos;s sexual life is present. This data property was inspired by the &quot;dpv:Sexual&quot; class in the Data Privacy Vocabulary (DPV).</rdfs:comment>
        <rdfs:seeAlso>https://www.w3.org/ns/dpv#dpv:Sexual</rdfs:seeAlso>
    </owl:DatatypeProperty>
    


    <!-- https://www.scss.tcd.ie/~kamarajk/EthicsOntology#hasSignedNDA -->

    <owl:DatatypeProperty rdf:about="https://www.scss.tcd.ie/~kamarajk/EthicsOntology#hasSignedNDA">
        <rdfs:domain rdf:resource="https://www.scss.tcd.ie/~kamarajk/EthicsOntology#Individual"/>
        <rdfs:range rdf:resource="http://www.w3.org/2001/XMLSchema#boolean"/>
        <rdfs:comment xml:lang="en">Information about any Non-disclosure agreements (NDA) that the data subject may have signed is present. This data property was inspired by the &quot;dpv:NDA&quot; class in the Data Privacy Vocabulary (DPV).</rdfs:comment>
        <rdfs:seeAlso>https://www.w3.org/ns/dpv#dpv:NDA</rdfs:seeAlso>
    </owl:DatatypeProperty>
    


    <!-- https://www.scss.tcd.ie/~kamarajk/EthicsOntology#hasTooManyDataPoints -->

    <owl:DatatypeProperty rdf:about="https://www.scss.tcd.ie/~kamarajk/EthicsOntology#hasTooManyDataPoints">
        <rdfs:domain rdf:resource="https://www.scss.tcd.ie/~kamarajk/EthicsOntology#Individual"/>
        <rdfs:range rdf:resource="http://www.w3.org/2001/XMLSchema#boolean"/>
        <rdfs:comment xml:lang="en">Too much of the data subject&apos;s data is present in the dataset.</rdfs:comment>
    </owl:DatatypeProperty>
    


    <!-- https://www.scss.tcd.ie/~kamarajk/EthicsOntology#hasUserTrackingData -->

    <owl:DatatypeProperty rdf:about="https://www.scss.tcd.ie/~kamarajk/EthicsOntology#hasUserTrackingData">
        <rdfs:domain rdf:resource="https://www.scss.tcd.ie/~kamarajk/EthicsOntology#Group"/>
        <rdfs:domain rdf:resource="https://www.scss.tcd.ie/~kamarajk/EthicsOntology#Individual"/>
        <rdfs:range rdf:resource="http://www.w3.org/2001/XMLSchema#boolean"/>
        <rdfs:comment xml:lang="en">Data that is related to tracking the data subject (online or offline) is present. This data property was inspired by the &quot;dpv:Tracking&quot; class in the Data Privacy Vocabulary (DPV).</rdfs:comment>
        <rdfs:seeAlso>https://www.w3.org/ns/dpv#dpv:Tracking</rdfs:seeAlso>
    </owl:DatatypeProperty>
    


    <!-- https://www.scss.tcd.ie/~kamarajk/EthicsOntology#isChild -->

    <owl:DatatypeProperty rdf:about="https://www.scss.tcd.ie/~kamarajk/EthicsOntology#isChild">
        <rdfs:domain rdf:resource="https://www.scss.tcd.ie/~kamarajk/EthicsOntology#Group"/>
        <rdfs:domain rdf:resource="https://www.scss.tcd.ie/~kamarajk/EthicsOntology#Individual"/>
        <rdfs:range rdf:resource="http://www.w3.org/2001/XMLSchema#boolean"/>
        <rdfs:comment xml:lang="en">The data subject is a child. This data property was inspired by the &quot;dpv:Child&quot; class in the Data Privacy Vocabulary (DPV).

According to DPV:

- A &apos;child&apos; is a natural legal person who is below a certain legal age depending on the legal jurisdiction.

- A &apos;child&apos; is distinct from a &apos;minor&apos;. For example, the legal age for a &apos;minor&apos; in most countries is 18, whereas a &apos;child&apos; can be a minor below the age of 14.</rdfs:comment>
        <rdfs:seeAlso>https://www.w3.org/ns/dpv#dpv:Child</rdfs:seeAlso>
    </owl:DatatypeProperty>
    


    <!-- https://www.scss.tcd.ie/~kamarajk/EthicsOntology#isValidForProcessing -->

    <owl:DatatypeProperty rdf:about="https://www.scss.tcd.ie/~kamarajk/EthicsOntology#isValidForProcessing">
        <rdfs:domain rdf:resource="https://w3id.org/GConsent#Status"/>
        <rdfs:range rdf:resource="http://www.w3.org/2001/XMLSchema#boolean"/>
        <rdfs:seeAlso xml:lang="en">The given consent renders the data as valid for processing by the current data controller. This data property was inspired by the &quot;Status valid for Processing&quot; class in GConsent.</rdfs:seeAlso>
        <rdfs:seeAlso>https://w3id.org/GConsent#StatusValidForProcessing</rdfs:seeAlso>
    </owl:DatatypeProperty>
    


    <!-- 
    ///////////////////////////////////////////////////////////////////////////////////////
    //
    // Classes
    //
    ///////////////////////////////////////////////////////////////////////////////////////
     -->

    


    <!-- http://www.w3.org/ns/dpv#dpv:DataController -->

    <owl:Class rdf:about="http://www.w3.org/ns/dpv#dpv:DataController">
        <rdfs:label xml:lang="en">Data Controller</rdfs:label>
    </owl:Class>
    


    <!-- http://www.w3.org/ns/dpv#dpv:DataSubject -->

    <owl:Class rdf:about="http://www.w3.org/ns/dpv#dpv:DataSubject">
        <rdfs:label xml:lang="en">Data Subject</rdfs:label>
    </owl:Class>
    


    <!-- https://w3id.org/GConsent#Consent -->

    <owl:Class rdf:about="https://w3id.org/GConsent#Consent"/>
    


    <!-- https://w3id.org/GConsent#Status -->

    <owl:Class rdf:about="https://w3id.org/GConsent#Status"/>
    


    <!-- https://www.scss.tcd.ie/~kamarajk/EthicsOntology#Group -->

    <owl:Class rdf:about="https://www.scss.tcd.ie/~kamarajk/EthicsOntology#Group">
        <rdfs:subClassOf rdf:resource="http://www.w3.org/ns/dpv#dpv:DataSubject"/>
        <owl:disjointWith rdf:resource="https://www.scss.tcd.ie/~kamarajk/EthicsOntology#Individual"/>
        <rdfs:comment xml:lang="en">Describes the data subject when it is a group, that is when the dataset represents different races, religions, or people with a certain disability.</rdfs:comment>
    </owl:Class>
    


    <!-- https://www.scss.tcd.ie/~kamarajk/EthicsOntology#Individual -->

    <owl:Class rdf:about="https://www.scss.tcd.ie/~kamarajk/EthicsOntology#Individual">
        <rdfs:subClassOf rdf:resource="http://www.w3.org/ns/dpv#dpv:DataSubject"/>
        <rdfs:comment xml:lang="en">Describes the data subject when it is an individual, that is when the dataset represents specific people.</rdfs:comment>
    </owl:Class>
</rdf:RDF>



<!-- Generated by the OWL API (version 4.5.9.2019-02-01T07:24:44Z) https://github.com/owlcs/owlapi -->

