@prefix : <https://www.scss.tcd.ie/~kamarajk/EthicsOntology#> .
@prefix owl: <http://www.w3.org/2002/07/owl#> .
@prefix rdf: <http://www.w3.org/1999/02/22-rdf-syntax-ns#> .
@prefix xml: <http://www.w3.org/XML/1998/namespace> .
@prefix xsd: <http://www.w3.org/2001/XMLSchema#> .
@prefix rdfs: <http://www.w3.org/2000/01/rdf-schema#> .
@base <https://www.scss.tcd.ie/~kamarajk/EthicsOntology> .

<https://www.scss.tcd.ie/~kamarajk/EthicsOntology> rdf:type owl:Ontology .

#################################################################
#    Object Properties
#################################################################

###  https://w3id.org/GConsent#hasConsent
<https://w3id.org/GConsent#hasConsent> rdf:type owl:ObjectProperty ;
                                       owl:inverseOf <https://w3id.org/GConsent#isConsentForDataSubject> ;
                                       rdfs:domain <http://www.w3.org/ns/dpv#dpv:DataSubject> ;
                                       rdfs:range <https://w3id.org/GConsent#Consent> .


###  https://w3id.org/GConsent#isConsentForDataSubject
<https://w3id.org/GConsent#isConsentForDataSubject> rdf:type owl:ObjectProperty ;
                                                    rdfs:domain <https://w3id.org/GConsent#Consent> ;
                                                    rdfs:range <http://www.w3.org/ns/dpv#dpv:DataSubject> .


###  https://w3id.org/GConsent#isProvidedToController
<https://w3id.org/GConsent#isProvidedToController> rdf:type owl:ObjectProperty ;
                                                   owl:inverseOf <https://w3id.org/GConsent#wasProvidedConsent> ;
                                                   rdf:type owl:InverseFunctionalProperty ,
                                                            owl:AsymmetricProperty ,
                                                            owl:IrreflexiveProperty ;
                                                   rdfs:domain <https://w3id.org/GConsent#Consent> ;
                                                   rdfs:range <http://www.w3.org/ns/dpv#dpv:DataController> .


###  https://w3id.org/GConsent#wasProvidedConsent
<https://w3id.org/GConsent#wasProvidedConsent> rdf:type owl:ObjectProperty ;
                                               rdfs:domain <http://www.w3.org/ns/dpv#dpv:DataController> ;
                                               rdfs:range <https://w3id.org/GConsent#Consent> .


###  https://www.scss.tcd.ie/~kamarajk/EthicsOntology#hasStatus
:hasStatus rdf:type owl:ObjectProperty ;
           owl:inverseOf :isStatusForConsent ;
           rdfs:domain <https://w3id.org/GConsent#Consent> ;
           rdfs:range <https://w3id.org/GConsent#Status> .


###  https://www.scss.tcd.ie/~kamarajk/EthicsOntology#isStatusForConsent
:isStatusForConsent rdf:type owl:ObjectProperty ;
                    rdfs:domain <https://w3id.org/GConsent#Status> ;
                    rdfs:range <https://w3id.org/GConsent#Consent> .


#################################################################
#    Data properties
#################################################################

###  https://www.scss.tcd.ie/~kamarajk/EthicsOntology#hasAccent
:hasAccent rdf:type owl:DatatypeProperty ;
           rdfs:domain :Group ,
                       :Individual ;
           rdfs:range xsd:boolean ;
           rdfs:comment "Information about the data subject’s accent is present. This data property was inspired by the \"dpv:Accent\" class in the Data Privacy Vocabulary (DPV)."@en ;
           rdfs:seeAlso "https://www.w3.org/ns/dpv#accent" .


###  https://www.scss.tcd.ie/~kamarajk/EthicsOntology#hasAge
:hasAge rdf:type owl:DatatypeProperty ;
        rdfs:domain :Group ,
                    :Individual ;
        rdfs:range xsd:boolean ;
        rdfs:comment "Information about the data subject’s age is present. This data property was inspired by the \"dpv:Age\" class in the Data Privacy Vocabulary (DPV)."@en ;
        rdfs:seeAlso "https://www.w3.org/ns/dpv#dpv:Age" .


###  https://www.scss.tcd.ie/~kamarajk/EthicsOntology#hasBehaviourData
:hasBehaviourData rdf:type owl:DatatypeProperty ;
                  rdfs:domain :Individual ;
                  rdfs:range xsd:boolean ;
                  rdfs:comment "Information about the data subject's behaviour is present. This data property was inspired by the \"dpv:Behavioral\" class in the Data Privacy Vocabulary (DPV)."@en ;
                  rdfs:seeAlso "https://www.w3.org/ns/dpv#dpv:Behavioral" .


###  https://www.scss.tcd.ie/~kamarajk/EthicsOntology#hasBodyStatistics
:hasBodyStatistics rdf:type owl:DatatypeProperty ;
                   rdfs:domain :Group ,
                               :Individual ;
                   rdfs:range xsd:boolean ;
                   rdfs:comment "Information about the data subject's physical metrics such as height, weight, waist size is present."@en .


###  https://www.scss.tcd.ie/~kamarajk/EthicsOntology#hasContactInformation
:hasContactInformation rdf:type owl:DatatypeProperty ;
                       rdfs:domain :Individual ;
                       rdfs:range xsd:boolean ;
                       rdfs:comment "Information about the data subject's contact details is present. Example: telephone number or email address. This data property was inspired by the \"dpv:Contact\" class in the Data Privacy Vocabulary (DPV)."@en ;
                       rdfs:seeAlso "https://www.w3.org/ns/dpv#dpv:Contact" .


###  https://www.scss.tcd.ie/~kamarajk/EthicsOntology#hasCountryOfOrigin
:hasCountryOfOrigin rdf:type owl:DatatypeProperty ;
                    rdfs:domain :Group ,
                                :Individual ;
                    rdfs:range xsd:boolean ;
                    rdfs:comment "Information about the data subject's native country is present."@en .


###  https://www.scss.tcd.ie/~kamarajk/EthicsOntology#hasCriminalActivity
:hasCriminalActivity rdf:type owl:DatatypeProperty ;
                     rdfs:domain :Group ,
                                 :Individual ;
                     rdfs:range xsd:boolean ;
                     rdfs:comment "Information about the data subject's criminal activity is present. Example: criminal convictions or jail time. This data property was inspired by the \"dpv:Criminal\" class in the Data Privacy Vocabulary (DPV)."@en ;
                     rdfs:seeAlso "https://www.w3.org/ns/dpv#criminal" .


###  https://www.scss.tcd.ie/~kamarajk/EthicsOntology#hasDataControllerName
:hasDataControllerName rdf:type owl:DatatypeProperty ;
                       rdfs:domain <http://www.w3.org/ns/dpv#dpv:DataController> ;
                       rdfs:range xsd:string ;
                       rdfs:comment "Indicates the name of the data controller."@en .


###  https://www.scss.tcd.ie/~kamarajk/EthicsOntology#hasDateOfBirth
:hasDateOfBirth rdf:type owl:DatatypeProperty ;
                rdfs:domain :Individual ;
                rdfs:range xsd:boolean ;
                rdfs:comment "Information about the data subject's date of birth is present."@en .


###  https://www.scss.tcd.ie/~kamarajk/EthicsOntology#hasDoctorConsulationsInfo
:hasDoctorConsulationsInfo rdf:type owl:DatatypeProperty ;
                           rdfs:domain :Group ,
                                       :Individual ;
                           rdfs:range xsd:boolean ;
                           rdfs:comment "Information about the data subject's doctor consultations is present."@en .


###  https://www.scss.tcd.ie/~kamarajk/EthicsOntology#hasDoctorConsultationsData
:hasDoctorConsultationsData rdf:type owl:DatatypeProperty ;
                            rdfs:domain :Group ,
                                        :Individual ;
                            rdfs:range xsd:boolean ;
                            rdfs:comment "Information about the data subject's doctor consultations is present."@en .


###  https://www.scss.tcd.ie/~kamarajk/EthicsOntology#hasFilesWithPIIAttached
:hasFilesWithPIIAttached rdf:type owl:DatatypeProperty ;
                         rdfs:domain :Individual ;
                         rdfs:range xsd:boolean ;
                         rdfs:comment "Files with the data subject's personally identifiable information is attached to the dataset. Example: Resume, photos, scanned financial documents, scanned doctor's report."@en .


###  https://www.scss.tcd.ie/~kamarajk/EthicsOntology#hasHealthData
:hasHealthData rdf:type owl:DatatypeProperty ;
               rdfs:domain :Group ,
                           :Individual ;
               rdfs:range xsd:boolean ;
               rdfs:comment "Information about the data subject's health, medical conditions or health care (medical history, test results, etc.) is present. This data property was inspired by the \"dpv:MedicalHealth\" class in the Data Privacy Vocabulary (DPV)."@en ;
               rdfs:seeAlso "https://www.w3.org/ns/dpv#dpv:MedicalHealth" .


###  https://www.scss.tcd.ie/~kamarajk/EthicsOntology#hasImmigrantParents
:hasImmigrantParents rdf:type owl:DatatypeProperty ;
                     rdfs:domain :Group ,
                                 :Individual ;
                     rdfs:range xsd:boolean ;
                     rdfs:comment "Information about the data subject's parent's immigration status is present."@en .


###  https://www.scss.tcd.ie/~kamarajk/EthicsOntology#hasIncomeBracketData
:hasIncomeBracketData rdf:type owl:DatatypeProperty ;
                      rdfs:domain :Group ,
                                  :Individual ;
                      rdfs:range xsd:boolean ;
                      rdfs:comment "Information about the data subject's income bracket is present. This data property was inspired by the \"dpv:IncomeBracket\" class in the Data Privacy Vocabulary (DPV)."@en ;
                      rdfs:seeAlso "https://www.w3.org/ns/dpv#income-bracket"@en .


###  https://www.scss.tcd.ie/~kamarajk/EthicsOntology#hasIncomeData
:hasIncomeData rdf:type owl:DatatypeProperty ;
               rdfs:domain :Individual ;
               rdfs:range xsd:boolean ;
               rdfs:comment "Information about the data subject's income is present. This data property was inspired by the \"dpv:Income\" class in the Data Privacy Vocabulary (DPV)."@en ;
               rdfs:seeAlso "https://www.w3.org/ns/dpv#income" .


###  https://www.scss.tcd.ie/~kamarajk/EthicsOntology#hasLanguageInformation
:hasLanguageInformation rdf:type owl:DatatypeProperty ;
                        rdfs:domain :Group ,
                                    :Individual ;
                        rdfs:range xsd:boolean ;
                        rdfs:comment "Information related to the data subject's language is present. This data property was inspired by the \"dpv:Language\" class in the Data Privacy Vocabulary (DPV)."@en ;
                        rdfs:seeAlso "https://www.w3.org/ns/dpv#dpv:Language" .


###  https://www.scss.tcd.ie/~kamarajk/EthicsOntology#hasLastName
:hasLastName rdf:type owl:DatatypeProperty ;
             rdfs:domain :Individual ;
             rdfs:range xsd:boolean ;
             rdfs:comment "An individual's last name is present. In some cases it can be used to identify the cast, race, religion, or country the individual belongs too."@en .


###  https://www.scss.tcd.ie/~kamarajk/EthicsOntology#hasLoanRecords
:hasLoanRecords rdf:type owl:DatatypeProperty ;
                rdfs:domain :Group ,
                            :Individual ;
                rdfs:range xsd:boolean ;
                rdfs:comment "Information about the loans provided to the the data subject or other related information is present. This data property was inspired by the \"dpv:LoanRecord\" class in the Data Privacy Vocabulary (DPV)."@en ;
                rdfs:seeAlso "https://www.w3.org/ns/dpv#dpv:LoanRecord" .


###  https://www.scss.tcd.ie/~kamarajk/EthicsOntology#hasLocationData
:hasLocationData rdf:type owl:DatatypeProperty ;
                 rdfs:domain :Group ,
                             :Individual ;
                 rdfs:range xsd:boolean ;
                 rdfs:comment "Information about the data subject's location is present. This data property was inspired by the \"dpv:Location\" class in the Data Privacy Vocabulary (DPV)."@en ;
                 rdfs:seeAlso "https://www.w3.org/ns/dpv#dpv:Location" .


###  https://www.scss.tcd.ie/~kamarajk/EthicsOntology#hasName
:hasName rdf:type owl:DatatypeProperty ;
         rdfs:domain :Individual ;
         rdfs:range xsd:boolean ;
         rdfs:comment "Information about the data subject's name is present. This data property was inspired by the \"dpv:Name\" class in the Data Privacy Vocabulary (DPV)."@en ;
         rdfs:seeAlso "https://www.w3.org/ns/dpv#dpv:Name" .


###  https://www.scss.tcd.ie/~kamarajk/EthicsOntology#hasPhysicalCharacteristics
:hasPhysicalCharacteristics rdf:type owl:DatatypeProperty ;
                            rdfs:domain :Group ,
                                        :Individual ;
                            rdfs:range xsd:boolean ;
                            rdfs:comment "Information about the data subject's physical characteristics is present. Example: handicapped, skin colour, hair colour, tattoos, piercings. This data property was inspired by the \"dpv:PhysicalCharacteristic\" class in the Data Privacy Vocabulary (DPV)."@en ;
                            rdfs:seeAlso "https://www.w3.org/ns/dpv#dpv:PhysicalCharacteristic" .


###  https://www.scss.tcd.ie/~kamarajk/EthicsOntology#hasPoliticalOpinions
:hasPoliticalOpinions rdf:type owl:DatatypeProperty ;
                      rdfs:domain :Group ,
                                  :Individual ;
                      rdfs:range xsd:boolean ;
                      rdfs:comment "Information about the data subject's political opinions are present."@en .


###  https://www.scss.tcd.ie/~kamarajk/EthicsOntology#hasRace
:hasRace rdf:type owl:DatatypeProperty ;
         rdfs:domain :Group ,
                     :Individual ;
         rdfs:range xsd:boolean ;
         rdfs:comment "Information about the data subject's race is present. This data property was inspired by the \"dpv:Race\" class in the Data Privacy Vocabulary (DPV)."@en ;
         rdfs:seeAlso "https://www.w3.org/ns/dpv#dpv:Race" .


###  https://www.scss.tcd.ie/~kamarajk/EthicsOntology#hasReligion
:hasReligion rdf:type owl:DatatypeProperty ;
             rdfs:domain :Group ,
                         :Individual ;
             rdfs:range xsd:boolean ;
             rdfs:comment "Information about the data subject's religion, religious inclinations, and religious history is present. This data property was inspired by the \"dpv:Religion\" class in the Data Privacy Vocabulary (DPV)."@en ;
             rdfs:seeAlso "https://www.w3.org/ns/dpv#dpv:Religion" .


###  https://www.scss.tcd.ie/~kamarajk/EthicsOntology#hasSexualData
:hasSexualData rdf:type owl:DatatypeProperty ;
               rdfs:domain :Group ,
                           :Individual ;
               rdfs:range xsd:boolean ;
               rdfs:comment "Information that describes the data subject's sexual life is present. This data property was inspired by the \"dpv:Sexual\" class in the Data Privacy Vocabulary (DPV)."@en ;
               rdfs:seeAlso "https://www.w3.org/ns/dpv#dpv:Sexual" .


###  https://www.scss.tcd.ie/~kamarajk/EthicsOntology#hasSignedNDA
:hasSignedNDA rdf:type owl:DatatypeProperty ;
              rdfs:domain :Individual ;
              rdfs:range xsd:boolean ;
              rdfs:comment "Information about any Non-disclosure agreements (NDA) that the data subject may have signed is present. This data property was inspired by the \"dpv:NDA\" class in the Data Privacy Vocabulary (DPV)."@en ;
              rdfs:seeAlso "https://www.w3.org/ns/dpv#dpv:NDA" .


###  https://www.scss.tcd.ie/~kamarajk/EthicsOntology#hasTooManyDataPoints
:hasTooManyDataPoints rdf:type owl:DatatypeProperty ;
                      rdfs:domain :Individual ;
                      rdfs:range xsd:boolean ;
                      rdfs:comment "Too much of the data subject's data is present in the dataset."@en .


###  https://www.scss.tcd.ie/~kamarajk/EthicsOntology#hasUserTrackingData
:hasUserTrackingData rdf:type owl:DatatypeProperty ;
                     rdfs:domain :Group ,
                                 :Individual ;
                     rdfs:range xsd:boolean ;
                     rdfs:comment "Data that is related to tracking the data subject (online or offline) is present. This data property was inspired by the \"dpv:Tracking\" class in the Data Privacy Vocabulary (DPV)."@en ;
                     rdfs:seeAlso "https://www.w3.org/ns/dpv#dpv:Tracking" .


###  https://www.scss.tcd.ie/~kamarajk/EthicsOntology#isChild
:isChild rdf:type owl:DatatypeProperty ;
         rdfs:domain :Group ,
                     :Individual ;
         rdfs:range xsd:boolean ;
         rdfs:comment """The data subject is a child. This data property was inspired by the \"dpv:Child\" class in the Data Privacy Vocabulary (DPV).

According to DPV:

- A 'child' is a natural legal person who is below a certain legal age depending on the legal jurisdiction.

- A 'child' is distinct from a 'minor'. For example, the legal age for a 'minor' in most countries is 18, whereas a 'child' can be a minor below the age of 14."""@en ;
         rdfs:seeAlso "https://www.w3.org/ns/dpv#dpv:Child" .


###  https://www.scss.tcd.ie/~kamarajk/EthicsOntology#isValidForProcessing
:isValidForProcessing rdf:type owl:DatatypeProperty ;
                      rdfs:domain <https://w3id.org/GConsent#Status> ;
                      rdfs:range xsd:boolean ;
                      rdfs:seeAlso "The given consent renders the data as valid for processing by the current data controller. This data property was inspired by the \"Status valid for Processing\" class in GConsent."@en ,
                                   "https://w3id.org/GConsent#StatusValidForProcessing" .


#################################################################
#    Classes
#################################################################

###  http://www.w3.org/ns/dpv#dpv:DataController
<http://www.w3.org/ns/dpv#dpv:DataController> rdf:type owl:Class ;
                                              rdfs:label "Data Controller"@en .


###  http://www.w3.org/ns/dpv#dpv:DataSubject
<http://www.w3.org/ns/dpv#dpv:DataSubject> rdf:type owl:Class ;
                                           rdfs:label "Data Subject"@en .


###  https://w3id.org/GConsent#Consent
<https://w3id.org/GConsent#Consent> rdf:type owl:Class .


###  https://w3id.org/GConsent#Status
<https://w3id.org/GConsent#Status> rdf:type owl:Class .


###  https://www.scss.tcd.ie/~kamarajk/EthicsOntology#Group
:Group rdf:type owl:Class ;
       rdfs:subClassOf <http://www.w3.org/ns/dpv#dpv:DataSubject> ;
       owl:disjointWith :Individual ;
       rdfs:comment "Describes the data subject when it is a group, that is when the dataset represents different races, religions, or people with a certain disability."@en .


###  https://www.scss.tcd.ie/~kamarajk/EthicsOntology#Individual
:Individual rdf:type owl:Class ;
            rdfs:subClassOf <http://www.w3.org/ns/dpv#dpv:DataSubject> ;
            rdfs:comment "Describes the data subject when it is an individual, that is when the dataset represents specific people."@en .


###  Generated by the OWL API (version 4.5.9.2019-02-01T07:24:44Z) https://github.com/owlcs/owlapi
