<?xml version="1.0" encoding="UTF-8"?>
<rdf:RDF
   xmlns="https://www.scss.tcd.ie/~kamarajk/EthicsOntology#"
   xmlns:owl="http://www.w3.org/2002/07/owl#"
   xmlns:rdf="http://www.w3.org/1999/02/22-rdf-syntax-ns#"
   xmlns:rdfs="http://www.w3.org/2000/01/rdf-schema#"
   xmlns:terms="http://purl.org/dc/terms/"
>
  <rdf:Description rdf:nodeID="Nd1d2b0b6c45e49adbe8d513971ba61be">
    <rdf:rest rdf:resource="http://www.w3.org/1999/02/22-rdf-syntax-ns#nil"/>
    <rdf:first rdf:resource="https://www.scss.tcd.ie/~kamarajk/EthicsOntology#Individual"/>
  </rdf:Description>
  <rdf:Description rdf:about="https://www.scss.tcd.ie/~kamarajk/EthicsOntology#Vocab_TestDataset">
    <hasDataControllerName>tes</hasDataControllerName>
    <hasIncomeData rdf:datatype="http://www.w3.org/2001/XMLSchema#boolean">true</hasIncomeData>
    <hasUserTrackingData rdf:datatype="http://www.w3.org/2001/XMLSchema#boolean">true</hasUserTrackingData>
    <hasHealthData rdf:datatype="http://www.w3.org/2001/XMLSchema#boolean">true</hasHealthData>
    <rdf:type rdf:resource="http://www.w3.org/2002/07/owl#NamedIndividual"/>
    <hasLoanRecords rdf:datatype="http://www.w3.org/2001/XMLSchema#boolean">true</hasLoanRecords>
    <hasBehaviourData rdf:datatype="http://www.w3.org/2001/XMLSchema#boolean">true</hasBehaviourData>
    <hasReligion rdf:datatype="http://www.w3.org/2001/XMLSchema#boolean">true</hasReligion>
    <hasFilesWithPIIAttached rdf:datatype="http://www.w3.org/2001/XMLSchema#boolean">true</hasFilesWithPIIAttached>
    <hasChildData rdf:datatype="http://www.w3.org/2001/XMLSchema#boolean">false</hasChildData>
    <hasLocationData rdf:datatype="http://www.w3.org/2001/XMLSchema#boolean">true</hasLocationData>
    <hasTooManyDataPoints rdf:datatype="http://www.w3.org/2001/XMLSchema#boolean">false</hasTooManyDataPoints>
    <hasPhysicalCharacteristics rdf:datatype="http://www.w3.org/2001/XMLSchema#boolean">false</hasPhysicalCharacteristics>
    <isValidForProcessing rdf:datatype="http://www.w3.org/2001/XMLSchema#boolean">false</isValidForProcessing>
    <hasName rdf:datatype="http://www.w3.org/2001/XMLSchema#boolean">false</hasName>
    <hasPoliticalOpinions rdf:datatype="http://www.w3.org/2001/XMLSchema#boolean">true</hasPoliticalOpinions>
    <hasContactInformation rdf:datatype="http://www.w3.org/2001/XMLSchema#boolean">false</hasContactInformation>
    <rdf:type rdf:resource="https://www.scss.tcd.ie/~kamarajk/EthicsOntology#Group"/>
    <hasCriminalActivity rdf:datatype="http://www.w3.org/2001/XMLSchema#boolean">false</hasCriminalActivity>
    <hasSignedNDA rdf:datatype="http://www.w3.org/2001/XMLSchema#boolean">false</hasSignedNDA>
    <hasAge rdf:datatype="http://www.w3.org/2001/XMLSchema#boolean">true</hasAge>
    <hasEthnicityData rdf:datatype="http://www.w3.org/2001/XMLSchema#boolean">true</hasEthnicityData>
  </rdf:Description>
  <rdf:Description rdf:about="https://www.scss.tcd.ie/~kamarajk/EthicsOntology#isValidForProcessing">
    <rdfs:label>is valid for processing</rdfs:label>
    <rdfs:seeAlso>https://w3id.org/GConsent#StatusValidForProcessing</rdfs:seeAlso>
    <rdfs:domain rdf:resource="https://w3id.org/GConsent#Status"/>
    <rdf:type rdf:resource="http://www.w3.org/2002/07/owl#DatatypeProperty"/>
    <rdfs:comment xml:lang="en">The given consent renders the data as valid for processing by the current data controller. This data property was inspired by the "Status valid for Processing" class in GConsent.</rdfs:comment>
    <rdfs:range rdf:resource="http://www.w3.org/2001/XMLSchema#boolean"/>
  </rdf:Description>
  <rdf:Description rdf:about="https://www.scss.tcd.ie/~kamarajk/EthicsOntology#hasHealthData">
    <rdfs:label xml:lang="en">has health data</rdfs:label>
    <rdf:type rdf:resource="http://www.w3.org/2002/07/owl#DatatypeProperty"/>
    <rdfs:domain rdf:nodeID="N764cf9ce90534c21ba2fc7b099a4f743"/>
    <rdfs:seeAlso>https://www.w3.org/ns/dpv#dpv:MedicalHealth</rdfs:seeAlso>
    <rdfs:comment xml:lang="en">Information about the data subject's health, medical conditions, doctor consultations or health care (medical history, test results, etc.) is present. This data property was inspired by the "dpv:MedicalHealth" class in the Data Privacy Vocabulary (DPV).</rdfs:comment>
    <rdfs:range rdf:resource="http://www.w3.org/2001/XMLSchema#boolean"/>
  </rdf:Description>
  <rdf:Description rdf:about="https://www.scss.tcd.ie/~kamarajk/EthicsOntology#Individual">
    <rdf:type rdf:resource="http://www.w3.org/2002/07/owl#Class"/>
    <rdfs:subClassOf rdf:resource="http://www.w3.org/ns/dpv#DataSubject"/>
    <rdfs:label>Individual</rdfs:label>
    <rdfs:comment xml:lang="en">Describes the data subject when it is an individual, that is when the dataset represents specific people.</rdfs:comment>
  </rdf:Description>
  <rdf:Description rdf:nodeID="N71d161ce7568496ead5b01d50e173762">
    <rdf:type rdf:resource="http://www.w3.org/2002/07/owl#Class"/>
    <owl:unionOf rdf:nodeID="N1c509552f816402aacba435ef72ff122"/>
  </rdf:Description>
  <rdf:Description rdf:nodeID="N8b312311dcf84bd99c1dc216df2bc151">
    <rdf:rest rdf:resource="http://www.w3.org/1999/02/22-rdf-syntax-ns#nil"/>
    <rdf:first rdf:resource="https://www.scss.tcd.ie/~kamarajk/EthicsOntology#Individual"/>
  </rdf:Description>
  <rdf:Description rdf:about="https://www.scss.tcd.ie/~kamarajk/EthicsOntology#hasName">
    <rdfs:range rdf:resource="http://www.w3.org/2001/XMLSchema#boolean"/>
    <rdfs:domain rdf:resource="https://www.scss.tcd.ie/~kamarajk/EthicsOntology#Individual"/>
    <rdfs:comment xml:lang="en">Information about the data subject's name is present. This data property was inspired by the "dpv:Name" class in the Data Privacy Vocabulary (DPV).

In some cases, an individual's name can be used to identify the caste, race, religion, or country the individual belongs too.</rdfs:comment>
    <rdf:type rdf:resource="http://www.w3.org/2002/07/owl#DatatypeProperty"/>
    <rdfs:label xml:lang="en">has name</rdfs:label>
    <rdfs:seeAlso>https://www.w3.org/ns/dpv#dpv:Name</rdfs:seeAlso>
  </rdf:Description>
  <rdf:Description rdf:nodeID="N764cf9ce90534c21ba2fc7b099a4f743">
    <owl:unionOf rdf:nodeID="N9310915b20d146f085fbdd42617fb777"/>
    <rdf:type rdf:resource="http://www.w3.org/2002/07/owl#Class"/>
  </rdf:Description>
  <rdf:Description rdf:about="https://w3id.org/GConsent#isProvidedToController">
    <rdfs:range rdf:resource="http://www.w3.org/ns/dpv#DataController"/>
    <rdf:type rdf:resource="http://www.w3.org/2002/07/owl#InverseFunctionalProperty"/>
    <rdf:type rdf:resource="http://www.w3.org/2002/07/owl#IrreflexiveProperty"/>
    <rdfs:comment xml:lang="en">Indicates the Organisation the consent was provided to.</rdfs:comment>
    <rdfs:domain rdf:resource="https://w3id.org/GConsent#Consent"/>
    <rdf:type rdf:resource="http://www.w3.org/2002/07/owl#AsymmetricProperty"/>
    <rdfs:label xml:lang="en">is provided to controller</rdfs:label>
    <owl:inverseOf rdf:resource="https://w3id.org/GConsent#wasProvidedConsent"/>
    <rdf:type rdf:resource="http://www.w3.org/2002/07/owl#ObjectProperty"/>
  </rdf:Description>
  <rdf:Description rdf:about="https://www.scss.tcd.ie/~kamarajk/EthicsOntology#Group">
    <rdfs:label>Group</rdfs:label>
    <owl:disjointWith rdf:resource="https://www.scss.tcd.ie/~kamarajk/EthicsOntology#Individual"/>
    <rdfs:subClassOf rdf:resource="http://www.w3.org/ns/dpv#DataSubject"/>
    <rdfs:comment xml:lang="en">Describes the data subject when it is a group, that is when the dataset represents different races, religions, or people with a certain disability.</rdfs:comment>
    <rdf:type rdf:resource="http://www.w3.org/2002/07/owl#Class"/>
  </rdf:Description>
  <rdf:Description rdf:about="https://www.scss.tcd.ie/~kamarajk/EthicsOntology#hasChildData">
    <rdfs:range rdf:resource="http://www.w3.org/2001/XMLSchema#boolean"/>
    <rdfs:domain rdf:nodeID="N5d355e42fbe948229e87d4e0776a7481"/>
    <rdf:type rdf:resource="http://www.w3.org/2002/07/owl#DatatypeProperty"/>
    <rdfs:label xml:lang="en">has child data</rdfs:label>
    <rdfs:seeAlso xml:lang="en">https://www.w3.org/ns/dpv#dpv:Child</rdfs:seeAlso>
    <rdfs:comment xml:lang="en">Indicates that the dataset contains child-related data. This data property was inspired by the "dpv:Child" class in the Data Privacy Vocabulary (DPV).

According to DPV:

- A 'child' is a natural legal person who is below a certain legal age depending on the legal jurisdiction.

- A 'child' is distinct from a 'minor'. For example, the legal age for a 'minor' in most countries is 18, whereas a 'child' can be a minor below the age of 14.</rdfs:comment>
  </rdf:Description>
  <rdf:Description rdf:about="https://www.scss.tcd.ie/~kamarajk/EthicsOntology#hasLocationData">
    <rdfs:label xml:lang="en">has location data</rdfs:label>
    <rdfs:range rdf:resource="http://www.w3.org/2001/XMLSchema#boolean"/>
    <rdfs:seeAlso>https://www.w3.org/ns/dpv#dpv:Location</rdfs:seeAlso>
    <rdfs:domain rdf:nodeID="N2d39a15d5e77424c83c6542ae95d4a72"/>
    <rdfs:comment xml:lang="en">Information about the data subject's location is present. This data property was inspired by the "dpv:Location" class in the Data Privacy Vocabulary (DPV).</rdfs:comment>
    <rdf:type rdf:resource="http://www.w3.org/2002/07/owl#DatatypeProperty"/>
  </rdf:Description>
  <rdf:Description rdf:about="https://www.scss.tcd.ie/~kamarajk/EthicsOntology#hasPoliticalOpinions">
    <rdfs:label xml:lang="en">has political opinions</rdfs:label>
    <rdfs:range rdf:resource="http://www.w3.org/2001/XMLSchema#boolean"/>
    <rdfs:domain rdf:nodeID="N809990b623134766ad8d6a9748a270f7"/>
    <rdfs:comment xml:lang="en">Information about the data subject's political opinions are present.</rdfs:comment>
    <rdf:type rdf:resource="http://www.w3.org/2002/07/owl#DatatypeProperty"/>
  </rdf:Description>
  <rdf:Description rdf:nodeID="Ne14ecaf4a5f743d4bcd8c0ce012fb657">
    <owl:unionOf rdf:nodeID="Ncabf29dc506449d4b602abc7c5fd6176"/>
    <rdf:type rdf:resource="http://www.w3.org/2002/07/owl#Class"/>
  </rdf:Description>
  <rdf:Description rdf:nodeID="N5b0de03e4f6440d2a554883a092fa82e">
    <rdf:rest rdf:nodeID="N3fcca206835d4a0b9f1345cced2cf49f"/>
    <rdf:first rdf:resource="https://www.scss.tcd.ie/~kamarajk/EthicsOntology#Group"/>
  </rdf:Description>
  <rdf:Description rdf:about="http://www.w3.org/ns/dpv#DataSubject">
    <terms:creator>Axel Polleres, Javier Ferenandez</terms:creator>
    <terms:created>2019-04-04</terms:created>
    <rdfs:label xml:lang="en">Data Subject</rdfs:label>
    <rdfs:comment xml:lang="en">The class of Data Subject that this particular data handling applies to, any legal entity that is defined by article 4.1 of GDPR.</rdfs:comment>
    <terms:date-accepted>2019-04-05</terms:date-accepted>
    <rdfs:isDefinedBy xml:lang="en">https://eur-lex.europa.eu/eli/reg/2016/679/art_4/par_1/pnt_g/oj</rdfs:isDefinedBy>
    <rdf:type rdf:resource="http://www.w3.org/2002/07/owl#Class"/>
  </rdf:Description>
  <rdf:Description rdf:nodeID="N5083080056fd4584a7565ee96fee2213">
    <rdf:rest rdf:nodeID="N99c7450d184d4f9e98f459b3043ff6d3"/>
    <rdf:first rdf:resource="https://www.scss.tcd.ie/~kamarajk/EthicsOntology#Group"/>
  </rdf:Description>
  <rdf:Description rdf:nodeID="Nfbe70de6d7db4b3fbad501ece898c579">
    <rdf:rest rdf:resource="http://www.w3.org/1999/02/22-rdf-syntax-ns#nil"/>
    <rdf:first rdf:resource="https://www.scss.tcd.ie/~kamarajk/EthicsOntology#Individual"/>
  </rdf:Description>
  <rdf:Description rdf:nodeID="N23251e82d5e94b52bbe1aba7afe95019">
    <rdf:rest rdf:nodeID="Nc908023bfe0f4282a8c3b612a2a69144"/>
    <rdf:first rdf:resource="https://www.scss.tcd.ie/~kamarajk/EthicsOntology#Group"/>
  </rdf:Description>
  <rdf:Description rdf:about="https://w3id.org/GConsent#wasProvidedConsent">
    <rdf:type rdf:resource="http://www.w3.org/2002/07/owl#ObjectProperty"/>
    <rdfs:label xml:lang="en">was provided consent</rdfs:label>
    <rdfs:domain rdf:resource="http://www.w3.org/ns/dpv#DataController"/>
    <rdfs:range rdf:resource="https://w3id.org/GConsent#Consent"/>
    <rdfs:comment xml:lang="en">Indicates that the specified Person or Data Controller was provided the associated consent.</rdfs:comment>
  </rdf:Description>
  <rdf:Description rdf:about="https://w3id.org/GConsent#isConsentForDataSubject">
    <rdfs:label xml:lang="en">is consent for data subject</rdfs:label>
    <rdfs:range rdf:resource="http://www.w3.org/ns/dpv#DataSubject"/>
    <rdfs:comment xml:lang="en">Links a consent instance with the data subject it is associated with.</rdfs:comment>
    <rdf:type rdf:resource="http://www.w3.org/2002/07/owl#ObjectProperty"/>
    <rdfs:domain rdf:resource="https://w3id.org/GConsent#Consent"/>
  </rdf:Description>
  <rdf:Description rdf:nodeID="Na27f3570f3164f379a268c3165f7f52d">
    <rdf:type rdf:resource="http://www.w3.org/2002/07/owl#Class"/>
    <owl:unionOf rdf:nodeID="N2a2447fab2704f85957f7db68ceba3c7"/>
  </rdf:Description>
  <rdf:Description rdf:nodeID="N94bff32b34bf4545b707ac967ee58366">
    <rdf:first rdf:resource="https://www.scss.tcd.ie/~kamarajk/EthicsOntology#Individual"/>
    <rdf:rest rdf:resource="http://www.w3.org/1999/02/22-rdf-syntax-ns#nil"/>
  </rdf:Description>
  <rdf:Description rdf:nodeID="N4579ff64b3694fa1908b7926f84ebbc8">
    <rdf:type rdf:resource="http://www.w3.org/2002/07/owl#Class"/>
    <owl:unionOf rdf:nodeID="N5b0de03e4f6440d2a554883a092fa82e"/>
  </rdf:Description>
  <rdf:Description rdf:nodeID="N1418f6bd06804615a563c07c8062346e">
    <rdf:first rdf:resource="https://www.scss.tcd.ie/~kamarajk/EthicsOntology#Individual"/>
    <rdf:rest rdf:resource="http://www.w3.org/1999/02/22-rdf-syntax-ns#nil"/>
  </rdf:Description>
  <rdf:Description rdf:about="https://w3id.org/GConsent#Consent">
    <rdfs:subClassOf rdf:nodeID="Nc3fbd04891fc473e8b97032cbcd19c71"/>
    <rdfs:isDefinedBy rdf:resource="https://w3id.org/GDPRtEXT#GivenConsent"/>
    <rdfs:subClassOf rdf:nodeID="N181fd50e8e9d4cb79fa116330fb380a7"/>
    <rdfs:comment>As per Article 4(11) of the GDPR, ‘consent’ of the data subject means any freely given, specific, informed and unambiguous indication of the data subject’s wishes by which he or she, by a statement or by a clear affirmative action, signifies agreement to the processing of personal data relating to him or her; In the case of this ontology, 'Consent' is a concept as well as a tangible entity (something that has a provenance record). To separate this distinction with relation to the data subject, the Consent class represents the consent of the data subject in its entirely, including any history and annotations for it. To link the `Consent` instance with the `DataSubject` instance, use the `isConsentForDataSubject` and `hasConsent` properties.</rdfs:comment>
    <rdfs:label>Consent</rdfs:label>
    <rdf:type rdf:resource="http://www.w3.org/2002/07/owl#Class"/>
  </rdf:Description>
  <rdf:Description rdf:nodeID="Ncabf29dc506449d4b602abc7c5fd6176">
    <rdf:first rdf:resource="https://www.scss.tcd.ie/~kamarajk/EthicsOntology#Group"/>
    <rdf:rest rdf:nodeID="Naa9129e6ab2e4f908df469c559f2b6c5"/>
  </rdf:Description>
  <rdf:Description rdf:nodeID="N99c7450d184d4f9e98f459b3043ff6d3">
    <rdf:rest rdf:resource="http://www.w3.org/1999/02/22-rdf-syntax-ns#nil"/>
    <rdf:first rdf:resource="https://www.scss.tcd.ie/~kamarajk/EthicsOntology#Individual"/>
  </rdf:Description>
  <rdf:Description rdf:about="https://www.scss.tcd.ie/~kamarajk/EthicsOntology#hasAge">
    <rdf:type rdf:resource="http://www.w3.org/2002/07/owl#DatatypeProperty"/>
    <rdfs:comment xml:lang="en">Information about the data subject’s age is present. This data property was inspired by the "dpv:Age" class in the Data Privacy Vocabulary (DPV).</rdfs:comment>
    <rdfs:seeAlso>https://www.w3.org/ns/dpv#dpv:Age</rdfs:seeAlso>
    <rdfs:range rdf:resource="http://www.w3.org/2001/XMLSchema#boolean"/>
    <rdfs:domain rdf:nodeID="N602c2ccdd7c54adc831661e50dd5392b"/>
    <rdfs:label xml:lang="en">has age</rdfs:label>
  </rdf:Description>
  <rdf:Description rdf:nodeID="Nbdbda5f64fa5448ea324a36bf7b3524e">
    <rdf:first rdf:resource="https://www.scss.tcd.ie/~kamarajk/EthicsOntology#Individual"/>
    <rdf:rest rdf:resource="http://www.w3.org/1999/02/22-rdf-syntax-ns#nil"/>
  </rdf:Description>
  <rdf:Description rdf:nodeID="N181fd50e8e9d4cb79fa116330fb380a7">
    <owl:qualifiedCardinality rdf:datatype="http://www.w3.org/2001/XMLSchema#nonNegativeInteger">1</owl:qualifiedCardinality>
    <rdf:type rdf:resource="http://www.w3.org/2002/07/owl#Restriction"/>
    <owl:onClass rdf:resource="https://w3id.org/GConsent#Status"/>
    <owl:onProperty rdf:resource="https://www.scss.tcd.ie/~kamarajk/EthicsOntology#hasStatus"/>
  </rdf:Description>
  <rdf:Description rdf:nodeID="Nc3fbd04891fc473e8b97032cbcd19c71">
    <owl:qualifiedCardinality rdf:datatype="http://www.w3.org/2001/XMLSchema#nonNegativeInteger">1</owl:qualifiedCardinality>
    <rdf:type rdf:resource="http://www.w3.org/2002/07/owl#Restriction"/>
    <owl:onClass rdf:resource="http://www.w3.org/ns/dpv#DataSubject"/>
    <owl:onProperty rdf:resource="https://w3id.org/GConsent#isConsentForDataSubject"/>
  </rdf:Description>
  <rdf:Description rdf:nodeID="Ndb881696377249e8b020696199602519">
    <owl:unionOf rdf:nodeID="Nb9e9e87a9cb64567b670f6bf218ece0b"/>
    <rdf:type rdf:resource="http://www.w3.org/2002/07/owl#Class"/>
  </rdf:Description>
  <rdf:Description rdf:nodeID="N1d328da4ec2e49e486f4c57229e9f639">
    <owl:unionOf rdf:nodeID="Nee39b239bb1c42b0b99592c0d074e75f"/>
    <rdf:type rdf:resource="http://www.w3.org/2002/07/owl#Class"/>
  </rdf:Description>
  <rdf:Description rdf:about="https://www.scss.tcd.ie/~kamarajk/EthicsOntology#isStatusForConsent">
    <rdfs:comment xml:lang="en">Links a status to the consent that uses it.</rdfs:comment>
    <rdfs:range rdf:resource="https://w3id.org/GConsent#Consent"/>
    <rdfs:domain rdf:resource="https://w3id.org/GConsent#Status"/>
    <rdfs:label xml:lang="en">is status for consent</rdfs:label>
    <rdf:type rdf:resource="http://www.w3.org/2002/07/owl#ObjectProperty"/>
  </rdf:Description>
  <rdf:Description rdf:about="https://www.scss.tcd.ie/~kamarajk/EthicsOntology#hasContactInformation">
    <rdfs:comment xml:lang="en">Information about the data subject's contact details is present. Example: telephone number or email address. This data property was inspired by the "dpv:Contact" class in the Data Privacy Vocabulary (DPV).</rdfs:comment>
    <rdf:type rdf:resource="http://www.w3.org/2002/07/owl#DatatypeProperty"/>
    <rdfs:seeAlso>https://www.w3.org/ns/dpv#dpv:Contact</rdfs:seeAlso>
    <rdfs:domain rdf:resource="https://www.scss.tcd.ie/~kamarajk/EthicsOntology#Individual"/>
    <rdfs:range rdf:resource="http://www.w3.org/2001/XMLSchema#boolean"/>
    <rdfs:label xml:lang="en">has contact information</rdfs:label>
  </rdf:Description>
  <rdf:Description rdf:about="https://www.scss.tcd.ie/~kamarajk/EthicsOntology#hasCriminalActivity">
    <rdfs:comment xml:lang="en">Information about the data subject's criminal activity is present. Example: criminal convictions or jail time. This data property was inspired by the "dpv:Criminal" class in the Data Privacy Vocabulary (DPV).</rdfs:comment>
    <rdf:type rdf:resource="http://www.w3.org/2002/07/owl#DatatypeProperty"/>
    <rdfs:label xml:lang="en">has criminal activity</rdfs:label>
    <rdfs:domain rdf:nodeID="Nbeec176d9932400aaafb3b9a6920a1f9"/>
    <rdfs:seeAlso>https://www.w3.org/ns/dpv#criminal</rdfs:seeAlso>
    <rdfs:range rdf:resource="http://www.w3.org/2001/XMLSchema#boolean"/>
  </rdf:Description>
  <rdf:Description rdf:about="https://w3id.org/GConsent#hasConsent">
    <rdfs:range rdf:resource="https://w3id.org/GConsent#Consent"/>
    <owl:inverseOf rdf:resource="https://w3id.org/GConsent#isConsentForDataSubject"/>
    <rdf:type rdf:resource="http://www.w3.org/2002/07/owl#ObjectProperty"/>
    <rdfs:domain rdf:resource="http://www.w3.org/ns/dpv#DataSubject"/>
    <rdfs:label xml:lang="en">has consent</rdfs:label>
    <rdfs:comment xml:lang="en">Links a data subject to their consent.</rdfs:comment>
    <rdfs:isDefinedBy rdf:resource="https://w3id.org/GDPRtEXT#Consent"/>
  </rdf:Description>
  <rdf:Description rdf:about="http://www.w3.org/ns/dpv#DataController">
    <terms:created>2019-04-04</terms:created>
    <rdfs:label xml:lang="en">Data Controller</rdfs:label>
    <rdf:type rdf:resource="http://www.w3.org/2002/07/owl#Class"/>
    <terms:creator>Axel Polleres, Javier Ferenandez</terms:creator>
    <rdfs:isDefinedBy rdf:resource="https://eur-lex.europa.eu/eli/reg/2016/679/art_4/par_7/pnt_g/oj"/>
    <terms:date-accepted>2019-04-05</terms:date-accepted>
    <rdfs:comment xml:lang="en">The class of Data Controllers that control this particular data handling, any legal entity that is defined by article 4.7 of GDPR.</rdfs:comment>
  </rdf:Description>
  <rdf:Description rdf:about="https://www.scss.tcd.ie/~kamarajk/EthicsOntology#hasIncomeData">
    <rdfs:domain rdf:nodeID="Nc2169d9c1bd24927b8e83dd0db788ea1"/>
    <rdfs:comment xml:lang="en">Information about the data subject's income or the income bracket in which they fit is present. This data property was inspired by the "dpv:Income" class in the Data Privacy Vocabulary (DPV).</rdfs:comment>
    <rdfs:seeAlso>https://www.w3.org/ns/dpv#income</rdfs:seeAlso>
    <rdfs:label xml:lang="en">has income data</rdfs:label>
    <rdfs:range rdf:resource="http://www.w3.org/2001/XMLSchema#boolean"/>
    <rdf:type rdf:resource="http://www.w3.org/2002/07/owl#DatatypeProperty"/>
  </rdf:Description>
  <rdf:Description rdf:about="https://www.scss.tcd.ie/~kamarajk/EthicsOntology#hasStatus">
    <rdf:type rdf:resource="http://www.w3.org/2002/07/owl#ObjectProperty"/>
    <owl:inverseOf rdf:resource="https://www.scss.tcd.ie/~kamarajk/EthicsOntology#isStatusForConsent"/>
    <rdfs:comment xml:lang="en">Denotes the state or status of consent.</rdfs:comment>
    <rdfs:domain rdf:resource="https://w3id.org/GConsent#Consent"/>
    <rdfs:range rdf:resource="https://w3id.org/GConsent#Status"/>
    <rdfs:label xml:lang="en">has status</rdfs:label>
  </rdf:Description>
  <rdf:Description rdf:about="https://www.scss.tcd.ie/~kamarajk/EthicsOntology#TestDataset">
    <hasEthnicityData rdf:datatype="http://www.w3.org/2001/XMLSchema#boolean">true</hasEthnicityData>
    <hasContactInformation rdf:datatype="http://www.w3.org/2001/XMLSchema#boolean">true</hasContactInformation>
    <hasChildData rdf:datatype="http://www.w3.org/2001/XMLSchema#boolean">false</hasChildData>
    <hasReligion rdf:datatype="http://www.w3.org/2001/XMLSchema#boolean">true</hasReligion>
    <hasTooManyDataPoints rdf:datatype="http://www.w3.org/2001/XMLSchema#boolean">true</hasTooManyDataPoints>
    <hasAge rdf:datatype="http://www.w3.org/2001/XMLSchema#boolean">true</hasAge>
    <rdf:type rdf:resource="https://www.scss.tcd.ie/~kamarajk/EthicsOntology#Individual"/>
    <hasBehaviourData rdf:datatype="http://www.w3.org/2001/XMLSchema#boolean">true</hasBehaviourData>
    <hasPoliticalOpinions rdf:datatype="http://www.w3.org/2001/XMLSchema#boolean">true</hasPoliticalOpinions>
    <hasCriminalActivity rdf:datatype="http://www.w3.org/2001/XMLSchema#boolean">true</hasCriminalActivity>
    <hasName rdf:datatype="http://www.w3.org/2001/XMLSchema#boolean">true</hasName>
    <isValidForProcessing rdf:datatype="http://www.w3.org/2001/XMLSchema#boolean">true</isValidForProcessing>
    <rdf:type rdf:resource="http://www.w3.org/2002/07/owl#NamedIndividual"/>
    <hasSignedNDA rdf:datatype="http://www.w3.org/2001/XMLSchema#boolean">false</hasSignedNDA>
    <hasLoanRecords rdf:datatype="http://www.w3.org/2001/XMLSchema#boolean">false</hasLoanRecords>
    <hasDataControllerName>test</hasDataControllerName>
    <hasPhysicalCharacteristics rdf:datatype="http://www.w3.org/2001/XMLSchema#boolean">true</hasPhysicalCharacteristics>
    <hasIncomeData rdf:datatype="http://www.w3.org/2001/XMLSchema#boolean">true</hasIncomeData>
    <hasUserTrackingData rdf:datatype="http://www.w3.org/2001/XMLSchema#boolean">true</hasUserTrackingData>
    <hasHealthData rdf:datatype="http://www.w3.org/2001/XMLSchema#boolean">true</hasHealthData>
    <hasFilesWithPIIAttached rdf:datatype="http://www.w3.org/2001/XMLSchema#boolean">false</hasFilesWithPIIAttached>
    <hasLocationData rdf:datatype="http://www.w3.org/2001/XMLSchema#boolean">true</hasLocationData>
  </rdf:Description>
  <rdf:Description rdf:about="https://www.scss.tcd.ie/~kamarajk/EthicsOntology#hasUserTrackingData">
    <rdf:type rdf:resource="http://www.w3.org/2002/07/owl#DatatypeProperty"/>
    <rdfs:domain rdf:nodeID="N1d328da4ec2e49e486f4c57229e9f639"/>
    <rdfs:label xml:lang="en">has user tracking data</rdfs:label>
    <rdfs:range rdf:resource="http://www.w3.org/2001/XMLSchema#boolean"/>
    <rdfs:seeAlso>https://www.w3.org/ns/dpv#dpv:Tracking</rdfs:seeAlso>
    <rdfs:comment xml:lang="en">Data that is related to tracking the data subject (online or offline) is present. This data property was inspired by the "dpv:Tracking" class in the Data Privacy Vocabulary (DPV).</rdfs:comment>
  </rdf:Description>
  <rdf:Description rdf:about="https://www.scss.tcd.ie/~kamarajk/EthicsOntology#hasEthnicityData">
    <rdf:type rdf:resource="http://www.w3.org/2002/07/owl#DatatypeProperty"/>
    <rdfs:domain rdf:nodeID="Na27f3570f3164f379a268c3165f7f52d"/>
    <rdfs:seeAlso>https://www.w3.org/ns/dpv#dpv:Ethnicity</rdfs:seeAlso>
    <rdfs:comment xml:lang="en">Information about the data subject’s origins and lineage is present. This data property was inspired by the "dpv:Ethnicity" class in the Data Privacy Vocabulary (DPV).

Ethicity data is any data that involves the data subject's ethnic origin, native language, race, caste, accent, dialect, or the immigration status of the data subject or their parents.</rdfs:comment>
    <rdfs:range rdf:resource="http://www.w3.org/2001/XMLSchema#boolean"/>
    <rdfs:label xml:lang="en">has ethnicity data</rdfs:label>
  </rdf:Description>
  <rdf:Description rdf:nodeID="N2a2447fab2704f85957f7db68ceba3c7">
    <rdf:rest rdf:nodeID="N94bff32b34bf4545b707ac967ee58366"/>
    <rdf:first rdf:resource="https://www.scss.tcd.ie/~kamarajk/EthicsOntology#Group"/>
  </rdf:Description>
  <rdf:Description rdf:about="http://purl.org/dc/terms/created">
    <rdf:type rdf:resource="http://www.w3.org/2002/07/owl#AnnotationProperty"/>
  </rdf:Description>
  <rdf:Description rdf:about="https://www.scss.tcd.ie/~kamarajk/EthicsOntology#hasTooManyDataPoints">
    <rdfs:label xml:lang="en">has too many data points</rdfs:label>
    <rdfs:comment xml:lang="en">Too much of the data subject's data is present in the dataset.</rdfs:comment>
    <rdfs:domain rdf:resource="https://www.scss.tcd.ie/~kamarajk/EthicsOntology#Individual"/>
    <rdfs:range rdf:resource="http://www.w3.org/2001/XMLSchema#boolean"/>
    <rdf:type rdf:resource="http://www.w3.org/2002/07/owl#DatatypeProperty"/>
  </rdf:Description>
  <rdf:Description rdf:nodeID="N3fcca206835d4a0b9f1345cced2cf49f">
    <rdf:rest rdf:resource="http://www.w3.org/1999/02/22-rdf-syntax-ns#nil"/>
    <rdf:first rdf:resource="https://www.scss.tcd.ie/~kamarajk/EthicsOntology#Individual"/>
  </rdf:Description>
  <rdf:Description rdf:about="https://www.scss.tcd.ie/~kamarajk/EthicsOntology#hasPhysicalCharacteristics">
    <rdfs:comment xml:lang="en">Information about the data subject's physical characteristics is present. Example: gender, physical disabilities, skin colour, hair colour, tattoos, piercings, body measurements. This data property was inspired by the "dpv:PhysicalCharacteristic" class in the Data Privacy Vocabulary (DPV).</rdfs:comment>
    <rdfs:seeAlso>https://www.w3.org/ns/dpv#dpv:PhysicalCharacteristic</rdfs:seeAlso>
    <rdfs:domain rdf:nodeID="Ne14ecaf4a5f743d4bcd8c0ce012fb657"/>
    <rdf:type rdf:resource="http://www.w3.org/2002/07/owl#DatatypeProperty"/>
    <rdfs:range rdf:resource="http://www.w3.org/2001/XMLSchema#boolean"/>
    <rdfs:label xml:lang="en">has physical characteristics</rdfs:label>
  </rdf:Description>
  <rdf:Description rdf:nodeID="N2d39a15d5e77424c83c6542ae95d4a72">
    <rdf:type rdf:resource="http://www.w3.org/2002/07/owl#Class"/>
    <owl:unionOf rdf:nodeID="N4674a20f02d54823a5b083eb50326b93"/>
  </rdf:Description>
  <rdf:Description rdf:nodeID="N496aca3532034fc8a0a142420c5f4d63">
    <rdf:rest rdf:resource="http://www.w3.org/1999/02/22-rdf-syntax-ns#nil"/>
    <rdf:first rdf:resource="https://www.scss.tcd.ie/~kamarajk/EthicsOntology#Individual"/>
  </rdf:Description>
  <rdf:Description rdf:about="https://www.scss.tcd.ie/~kamarajk/EthicsOntology#hasReligion">
    <rdfs:range rdf:resource="http://www.w3.org/2001/XMLSchema#boolean"/>
    <rdfs:domain rdf:nodeID="Ndb881696377249e8b020696199602519"/>
    <rdf:type rdf:resource="http://www.w3.org/2002/07/owl#DatatypeProperty"/>
    <rdfs:comment xml:lang="en">Information about the data subject's religion, religious inclinations, and religious history is present. This data property was inspired by the "dpv:Religion" class in the Data Privacy Vocabulary (DPV).</rdfs:comment>
    <rdfs:label xml:lang="en">has religion</rdfs:label>
    <rdfs:seeAlso>https://www.w3.org/ns/dpv#dpv:Religion</rdfs:seeAlso>
  </rdf:Description>
  <rdf:Description rdf:nodeID="N5d355e42fbe948229e87d4e0776a7481">
    <owl:unionOf rdf:nodeID="Nd0efa32bd28948e2b08ee13fd72409f3"/>
    <rdf:type rdf:resource="http://www.w3.org/2002/07/owl#Class"/>
  </rdf:Description>
  <rdf:Description rdf:about="https://www.scss.tcd.ie/~kamarajk/EthicsOntology#hasFilesWithPIIAttached">
    <rdfs:range rdf:resource="http://www.w3.org/2001/XMLSchema#boolean"/>
    <rdfs:label xml:lang="en">has files with PII attached</rdfs:label>
    <rdf:type rdf:resource="http://www.w3.org/2002/07/owl#DatatypeProperty"/>
    <rdfs:domain rdf:nodeID="N71d161ce7568496ead5b01d50e173762"/>
    <rdfs:comment xml:lang="en">Files with the data subject's personally identifiable information (PII) is attached to the dataset. Example: Resume, photos, scanned financial documents, scanned doctor's report, PDF containing sensitive details about the members of a group.</rdfs:comment>
  </rdf:Description>
  <rdf:Description rdf:nodeID="N02a07d99cb62441ea312ef56f4b0bace">
    <rdf:rest rdf:resource="http://www.w3.org/1999/02/22-rdf-syntax-ns#nil"/>
    <rdf:first rdf:resource="https://www.scss.tcd.ie/~kamarajk/EthicsOntology#Individual"/>
  </rdf:Description>
  <rdf:Description rdf:nodeID="Naa9129e6ab2e4f908df469c559f2b6c5">
    <rdf:rest rdf:resource="http://www.w3.org/1999/02/22-rdf-syntax-ns#nil"/>
    <rdf:first rdf:resource="https://www.scss.tcd.ie/~kamarajk/EthicsOntology#Individual"/>
  </rdf:Description>
  <rdf:Description rdf:nodeID="Ndd5935cf815b445cba8374dcd98c76ed">
    <rdf:first rdf:resource="https://www.scss.tcd.ie/~kamarajk/EthicsOntology#Individual"/>
    <rdf:rest rdf:resource="http://www.w3.org/1999/02/22-rdf-syntax-ns#nil"/>
  </rdf:Description>
  <rdf:Description rdf:about="https://www.scss.tcd.ie/~kamarajk/EthicsOntology#hasLoanRecords">
    <rdf:type rdf:resource="http://www.w3.org/2002/07/owl#DatatypeProperty"/>
    <rdfs:domain rdf:nodeID="N4579ff64b3694fa1908b7926f84ebbc8"/>
    <rdfs:seeAlso>https://www.w3.org/ns/dpv#dpv:LoanRecord</rdfs:seeAlso>
    <rdfs:label xml:lang="en">has loan records</rdfs:label>
    <rdfs:comment xml:lang="en">Information about the loans provided to the the data subject or other related information is present. This data property was inspired by the "dpv:LoanRecord" class in the Data Privacy Vocabulary (DPV).</rdfs:comment>
    <rdfs:range rdf:resource="http://www.w3.org/2001/XMLSchema#boolean"/>
  </rdf:Description>
  <rdf:Description rdf:nodeID="Nab32393af47b4463b82d3d7143f0a9ce">
    <rdf:first rdf:resource="https://www.scss.tcd.ie/~kamarajk/EthicsOntology#Individual"/>
    <rdf:rest rdf:resource="http://www.w3.org/1999/02/22-rdf-syntax-ns#nil"/>
  </rdf:Description>
  <rdf:Description rdf:nodeID="Nd0efa32bd28948e2b08ee13fd72409f3">
    <rdf:rest rdf:nodeID="Nd1d2b0b6c45e49adbe8d513971ba61be"/>
    <rdf:first rdf:resource="https://www.scss.tcd.ie/~kamarajk/EthicsOntology#Group"/>
  </rdf:Description>
  <rdf:Description rdf:nodeID="Nc2169d9c1bd24927b8e83dd0db788ea1">
    <rdf:type rdf:resource="http://www.w3.org/2002/07/owl#Class"/>
    <owl:unionOf rdf:nodeID="N11a307c019724f31b491d57a551fe13b"/>
  </rdf:Description>
  <rdf:Description rdf:nodeID="Nbeec176d9932400aaafb3b9a6920a1f9">
    <owl:unionOf rdf:nodeID="N5083080056fd4584a7565ee96fee2213"/>
    <rdf:type rdf:resource="http://www.w3.org/2002/07/owl#Class"/>
  </rdf:Description>
  <rdf:Description rdf:nodeID="N1d2f41f64fd84c6880581e5f6a645600">
    <rdf:type rdf:resource="http://www.w3.org/2002/07/owl#Class"/>
    <owl:unionOf rdf:nodeID="Neaf6c5bf4dd540039abc0665e91456ad"/>
  </rdf:Description>
  <rdf:Description rdf:about="https://www.scss.tcd.ie/~kamarajk/EthicsOntology">
    <terms:license rdf:resource="https://creativecommons.org/licenses/by/4.0/"/>
    <rdf:type rdf:resource="http://www.w3.org/2002/07/owl#Ontology"/>
  </rdf:Description>
  <rdf:Description rdf:nodeID="N9310915b20d146f085fbdd42617fb777">
    <rdf:rest rdf:nodeID="Ndd5935cf815b445cba8374dcd98c76ed"/>
    <rdf:first rdf:resource="https://www.scss.tcd.ie/~kamarajk/EthicsOntology#Group"/>
  </rdf:Description>
  <rdf:Description rdf:nodeID="Nee39b239bb1c42b0b99592c0d074e75f">
    <rdf:first rdf:resource="https://www.scss.tcd.ie/~kamarajk/EthicsOntology#Group"/>
    <rdf:rest rdf:nodeID="N8b312311dcf84bd99c1dc216df2bc151"/>
  </rdf:Description>
  <rdf:Description rdf:nodeID="Neaf6c5bf4dd540039abc0665e91456ad">
    <rdf:rest rdf:nodeID="Nfbe70de6d7db4b3fbad501ece898c579"/>
    <rdf:first rdf:resource="https://www.scss.tcd.ie/~kamarajk/EthicsOntology#Group"/>
  </rdf:Description>
  <rdf:Description rdf:about="https://www.scss.tcd.ie/~kamarajk/EthicsOntology#hasDataControllerName">
    <rdfs:label xml:lang="en">has data controller name</rdfs:label>
    <rdfs:domain rdf:resource="http://www.w3.org/ns/dpv#DataController"/>
    <rdfs:comment xml:lang="en">Indicates the name of the data controller.</rdfs:comment>
    <rdf:type rdf:resource="http://www.w3.org/2002/07/owl#DatatypeProperty"/>
    <rdfs:range rdf:resource="http://www.w3.org/2001/XMLSchema#string"/>
  </rdf:Description>
  <rdf:Description rdf:nodeID="N1c509552f816402aacba435ef72ff122">
    <rdf:rest rdf:nodeID="N02a07d99cb62441ea312ef56f4b0bace"/>
    <rdf:first rdf:resource="https://www.scss.tcd.ie/~kamarajk/EthicsOntology#Group"/>
  </rdf:Description>
  <rdf:Description rdf:about="https://w3id.org/GConsent#Status">
    <rdf:type rdf:resource="http://www.w3.org/2002/07/owl#Class"/>
    <rdfs:label>Status</rdfs:label>
    <rdfs:comment>Represents the status of consent for the data subject. This allows persisting the determination of the validatity or suitability of consent (as an entity or instance) for use in processing and other activities. Examples: consent is given, consent is requested but not given, consent was withdrawn.</rdfs:comment>
  </rdf:Description>
  <rdf:Description rdf:nodeID="Nc908023bfe0f4282a8c3b612a2a69144">
    <rdf:rest rdf:resource="http://www.w3.org/1999/02/22-rdf-syntax-ns#nil"/>
    <rdf:first rdf:resource="https://www.scss.tcd.ie/~kamarajk/EthicsOntology#Individual"/>
  </rdf:Description>
  <rdf:Description rdf:about="https://www.scss.tcd.ie/~kamarajk/EthicsOntology#hasSignedNDA">
    <rdfs:comment xml:lang="en">Information about any Non-disclosure agreements (NDA) that the data subject may have signed is present. This data property was inspired by the "dpv:NDA" class in the Data Privacy Vocabulary (DPV).</rdfs:comment>
    <rdfs:label xml:lang="en">has signed NDA</rdfs:label>
    <rdfs:range rdf:resource="http://www.w3.org/2001/XMLSchema#boolean"/>
    <rdfs:seeAlso>https://www.w3.org/ns/dpv#dpv:NDA</rdfs:seeAlso>
    <rdfs:domain rdf:resource="https://www.scss.tcd.ie/~kamarajk/EthicsOntology#Individual"/>
    <rdf:type rdf:resource="http://www.w3.org/2002/07/owl#DatatypeProperty"/>
  </rdf:Description>
  <rdf:Description rdf:about="https://www.scss.tcd.ie/~kamarajk/EthicsOntology#hasBehaviourData">
    <rdfs:label xml:lang="en">has behaviour data</rdfs:label>
    <rdfs:comment xml:lang="en">Information about the data subject's behaviour is present. This data property was inspired by the "dpv:Behavioral" class in the Data Privacy Vocabulary (DPV).</rdfs:comment>
    <rdfs:seeAlso>https://www.w3.org/ns/dpv#dpv:Behavioral</rdfs:seeAlso>
    <rdf:type rdf:resource="http://www.w3.org/2002/07/owl#DatatypeProperty"/>
    <rdfs:range rdf:resource="http://www.w3.org/2001/XMLSchema#boolean"/>
    <rdfs:domain rdf:nodeID="N1d2f41f64fd84c6880581e5f6a645600"/>
  </rdf:Description>
  <rdf:Description rdf:nodeID="N11a307c019724f31b491d57a551fe13b">
    <rdf:rest rdf:nodeID="Nab32393af47b4463b82d3d7143f0a9ce"/>
    <rdf:first rdf:resource="https://www.scss.tcd.ie/~kamarajk/EthicsOntology#Group"/>
  </rdf:Description>
  <rdf:Description rdf:nodeID="N29dbf6124247483e94ae585361f51aaf">
    <rdf:first rdf:resource="https://www.scss.tcd.ie/~kamarajk/EthicsOntology#Group"/>
    <rdf:rest rdf:nodeID="N496aca3532034fc8a0a142420c5f4d63"/>
  </rdf:Description>
  <rdf:Description rdf:about="http://purl.org/dc/terms/license">
    <rdf:type rdf:resource="http://www.w3.org/2002/07/owl#AnnotationProperty"/>
  </rdf:Description>
  <rdf:Description rdf:nodeID="Nb9e9e87a9cb64567b670f6bf218ece0b">
    <rdf:first rdf:resource="https://www.scss.tcd.ie/~kamarajk/EthicsOntology#Group"/>
    <rdf:rest rdf:nodeID="N1418f6bd06804615a563c07c8062346e"/>
  </rdf:Description>
  <rdf:Description rdf:about="http://purl.org/dc/terms/creator">
    <rdf:type rdf:resource="http://www.w3.org/2002/07/owl#AnnotationProperty"/>
  </rdf:Description>
  <rdf:Description rdf:nodeID="N602c2ccdd7c54adc831661e50dd5392b">
    <rdf:type rdf:resource="http://www.w3.org/2002/07/owl#Class"/>
    <owl:unionOf rdf:nodeID="N29dbf6124247483e94ae585361f51aaf"/>
  </rdf:Description>
  <rdf:Description rdf:nodeID="N809990b623134766ad8d6a9748a270f7">
    <owl:unionOf rdf:nodeID="N23251e82d5e94b52bbe1aba7afe95019"/>
    <rdf:type rdf:resource="http://www.w3.org/2002/07/owl#Class"/>
  </rdf:Description>
  <rdf:Description rdf:nodeID="N4674a20f02d54823a5b083eb50326b93">
    <rdf:first rdf:resource="https://www.scss.tcd.ie/~kamarajk/EthicsOntology#Group"/>
    <rdf:rest rdf:nodeID="Nbdbda5f64fa5448ea324a36bf7b3524e"/>
  </rdf:Description>
  <rdf:Description rdf:about="http://purl.org/dc/terms/description">
    <rdf:type rdf:resource="http://www.w3.org/2002/07/owl#AnnotationProperty"/>
  </rdf:Description>
  <rdf:Description rdf:about="http://purl.org/dc/terms/date-accepted">
    <rdf:type rdf:resource="http://www.w3.org/2002/07/owl#AnnotationProperty"/>
  </rdf:Description>
</rdf:RDF>
